proof of correctness for BFS

examples/graph/theories/BFSProofs.v
@@ -11,7 +11,9 @@ Require Import Coq.Lists.SetoidList.
 Require Import Omega.
 Require Import Wellfounded.
 Require Import Coq.Relations.Relation_Operators.
-Require Import Coq.Lists.ListDec.
+Require Import Path.
+Require Import Helper.
+Require Import Coq.FSets.FMapFacts.
 
 Require Import CoLoR.Util.Relation.Lexico.
 Require Import CoLoR.Util.Relation.SN.
@@ -21,98 +23,9 @@ Require Import Coq.FSets.FMapInterface.
 Require Import Coq.Structures.OrderedTypeEx.
 
 Module M := FMapList.Make(N_as_OT).
+Module P := WProperties_fun N_as_OT M.
+Module F := P.F.
 
-
-(*Helpers*)
-Definition null {a} (l: list a) :=
-  match l with
-  | nil => true
-  | _ => false
-  end.
-
-Ltac simplify' := try(rewrite andb_diag in *); try(rewrite andb_true_iff in *); try(rewrite negb_true_iff in *);
-  try(rewrite andb_false_iff in *); try(rewrite negb_false_iff in *); intuition.
-
-Ltac destruct_all :=
-repeat(match goal with
-            |[H: (exists _, _) |- _] => destruct H
-            |[H: _ /\ _ |- _] => destruct H 
-            end; try(rewrite andb_true_iff in *)).
-
-(*Ltac for solving statements of the form: In x l, where l may be many lists appended together*) 
-Ltac solve_in :=
-  match goal with
-  | [ H : _ |- In ?x (?l ++ ?r)] => apply in_or_app; solve_in
-  | [ H : _ |- In ?x ?s \/ In ?x ?s'] => (right; solve_in) + (left; solve_in) 
-  | [ H : _ |- In ?x (?x :: ?l)] => simpl; left; reflexivity
-  | [H : _ |- In ?x (?a :: ?l)] => simpl; right; solve_in
-  | [ H : _ |- _ ] => try(reflexivity); assumption
-end. 
-
-Lemma in_split_app_fst: forall (A: Type) (l: list A) (x: A),
-  (forall x y : A, {x = y} + {x <> y}) ->
-  In x l ->
-  exists l1 l2, l = l1 ++ (x :: l2) /\ forall y, In y l1 -> y <> x.
-Proof.
-  intros. induction l.
-  - inversion H.
-  - destruct (X x a). subst. exists nil. exists l. split. reflexivity. intros. inversion H0.
-    simpl in H. destruct H. subst. contradiction.  apply IHl in H. destruct_all.
-    exists (a :: x0). exists x1. split. rewrite H. reflexivity. intros. intro. subst.
-    simpl in H1. destruct H1. subst. contradiction. apply H0 in H. contradiction.
-Qed.
-
-Lemma no_no_dup: forall (A: Type) (l: list A),
-  (forall x y : A, {x = y} + {x <> y}) ->
-  ~(NoDup l) <-> (exists w l1 l2 l3, l = l1 ++ w :: l2 ++ w :: l3).
-Proof.
-  intros. split; intros.
-  - induction l.
-    + assert (@NoDup A nil). constructor. contradiction.
-    + destruct (NoDup_dec X l).
-      * assert (In a l). destruct (In_dec X a l). apply i.
-        assert (NoDup (a :: l)). constructor. apply n0. apply n. contradiction.
-        apply in_split_app_fst in H0. destruct_all. exists a. exists nil. exists x. exists x0.
-        rewrite H0. reflexivity. apply X.
-      * apply IHl in n. destruct_all. exists x. exists (a :: x0). exists x1. exists x2. rewrite H0.
-        reflexivity.
-  -  intro. destruct_all.  subst. induction x0; simpl in *.
-    + rewrite NoDup_cons_iff in H0. destruct_all. apply H.
-    solve_in.
-    + simpl in H0. rewrite NoDup_cons_iff in H0. destruct_all. apply IHx0. apply H0.
-Qed.
-
-
-(*
-(*Function to pop off queue satisfying given predicate*)
-Fixpoint pop_list {a} (l: list a) (p: a -> bool) :=
-  match l with
-  | nil => nil
-  | x :: xs => if (p x) then pop_list xs p else l
-  end.
-
-Definition pop_queue {a} (q: Queue.Queue a) (p: a -> bool) : Queue.Queue a :=
-  queuePutList (pop_list (toList _ q) p) mkQueue.
-
-(*Prove that first elt of queue satisfies predicate, prove for lists*)
-Lemma pop_list_split: forall {a} (l : list a) p,
- exists l1, l1 ++ (pop_list l p) = l /\ (forall x, In x l1 -> p x = true).
-Proof.
-  intros. induction l.
-  - exists nil. split; crush.
-  - simpl. destruct (p a0) eqn : B. destruct IHl. exists (a0 :: x). split. simpl. destruct H. rewrite <- H at 2.
-    reflexivity.
-    intros. simpl in H0. destruct H0. subst. assumption. apply H. assumption.
-    exists nil. split. reflexivity. intros. destruct H.
-Qed.
-
-Lemma pop_split_fst: forall {a} (l: list a) p h t,
-  pop_list l p = t :: h -> p t = false.
-Proof.
-  intros. induction l. simpl in H. inversion H. simpl in H. destruct (p a0) eqn : B.
-  apply IHl. apply H. inversion H; subst; assumption.
-Qed.
-*)
 (* Inductive relation*)
 Section Ind.
 
@@ -121,10 +34,10 @@ Context {a : Type} {b : Type} { gr : Type -> Type -> Type} {Hgraph : Graph.Graph
 Section Lex.
 
 (*Well formed lexicographic measure - maybe put in own section*)
-Definition natNodes (g : gr a b) := (BinInt.Z.abs_nat(Graph.noNodes g)).
+Definition natNodes := (@Path.natNodes a b gr Hgraph).
 
-Definition natNodes_lt x y := natNodes x < natNodes y.
-Definition natNodes_eq x y := natNodes x = natNodes y.
+Definition natNodes_lt (x y : gr a b) := natNodes x < natNodes y.
+Definition natNodes_eq (x y : gr a b) := natNodes x = natNodes y.
 Definition list_length_lt {a} (x y : list a) := length x < length y.
 Definition queue_length_lt  {a} (x y : Queue a) := list_length_lt (toList _ x) (toList _ y).
 
@@ -147,7 +60,6 @@ Lemma f_nat_lt_wf: forall {a} (f: a -> nat), well_founded (f_nat_lt f).
 Proof.
   red. intro. intro. intro. eapply f_nat_lt_acc. eauto.
 Qed.
-
 
 Lemma wf_bf_measure_list : forall a,  WF (transp (bf_measure_list a)).
 Proof.
@@ -187,58 +99,42 @@ Proof.
   apply WF_transp_wf. apply wf_bf_measure_queue.
 Qed.
 
-
-
-
 End Lex.
 
-Definition state : Type := (gr a b) * (list (Node * Num.Int)) * (list (Node * Num.Int)) * nat * (M.t nat).
-  
+Definition state : Type := (gr a b) * (list (Node * Num.Int)) * (list (Node * Num.Int)) .
+
 
 Definition get_graph (s: state) :=
   match s with
-  | (g, _, _, _, _) => g
+  | (g, _, _) => g
   end.
 
 Definition get_queue (s: state) :=
   match s with
-  | (_, q, _, _, _) => q
+  | (_, q, _) => q
 end.
 
 Definition get_dists (s: state) :=
   match s with
-  | (_, _, d, _, _) => d
+  | (_, _, d) => d
   end.
-
-Definition get_time (s: state) :=
-  match s with
-  | (_, _, _, t, _) => t
-  end.
-
-Definition get_times (s: state) :=
-  match s with
-  |(_, _, _, _, t) => t
-  end.
-
-Definition vertex_in (g: gr a b) (v: Graph.Node) : bool :=
-  match (Graph.match_ v g) with | (None, _) => false | _ => true end.
 
 Inductive bfs_step : state -> state -> Prop :=
-  | bfs_find: forall g d n t v j vs c g',
+  | bfs_find: forall g d v j vs c g',
       isEmpty g = false ->
       match_ v g = (Some c, g') ->
-      bfs_step (g, (v, j) :: vs, d, n, t) (g', (vs ++ suci c (Num.op_zp__ j (Num.fromInteger 1))),
-        d ++ (v,j) :: nil, n + 1, (M.add v (n+1) t))
-  | bfs_skip: forall g d n t v j vs g',
+      bfs_step (g, (v, j) :: vs, d) (g', (vs ++ suci c (Num.op_zp__ j (Num.fromInteger 1))),
+        d ++ (v,j) :: nil)
+  | bfs_skip: forall g d v j vs g',
       isEmpty g = false ->
       match_ v g = (None, g') ->
-      bfs_step (g, (v, j) :: vs, d, n, t) (g', vs, d, n, t).
+      bfs_step (g, (v, j) :: vs, d) (g', vs, d).
 
-Definition start (g : gr a b) (v: Graph.Node) : state := (g, ((v, Num.fromInteger 0) :: nil), nil, 0, @M.empty nat).
+Definition start (g : gr a b) (v: Graph.Node) : state := (g, ((v, Num.fromInteger 0) :: nil), nil).
 
-Inductive valid : state -> Node -> Prop :=
-  | v_start : forall g v, vertex_in g v = true -> valid (start g v) v
-  | v_step : forall s s' v, valid s' v -> bfs_step s' s -> valid s v.
+Inductive valid : state -> (gr a b) -> Node -> Prop :=
+  | v_start : forall g v, vIn g v = true -> valid (start g v) g v
+  | v_step : forall s s' v g, valid s' g v -> bfs_step s' s -> valid s g v.
 
 (*From Software Foundations*)
 Definition relation (X : Type) := X -> X -> Prop.
@@ -274,323 +170,38 @@ Qed.
 
 Definition bfs_multi (s1 s2 : state):= multi (bfs_step) s1 s2.
 
-Lemma multi_valid: forall s1 s2 v,
-  valid s1 v ->
+Lemma multi_valid: forall s1 s2 g v,
+  valid s1 g v ->
   bfs_multi s1 s2 ->
-  valid s2 v.
+  valid s2 g v.
 Proof.
   intros. induction H0. assumption. apply IHmulti. eapply v_step. apply H. assumption.
 Qed.
 
 Definition done (s: state) := null (get_queue s) || isEmpty (get_graph s).
 
-(*Proof of correctness of bfs. Later, we prove equivalence between this inductive formulation and leveln,
-  allowing us to prove the correctness of this instead*)
-Section Correctness.
+(*The executable, tail recursive version of this, which we will prove equivalent to the hs-to-coq version*)
+Section Exec.
 
-(*Lots of stuff about paths here - TODO: move to separate file*)
-Section Path.
-
-(*Inductive and Fixpoint definitions for a path between two vertices. The Fixpoint instance proves that this is
-  decidable, and we prove their equivalence*)
-Inductive path : (gr a b) -> Node -> Node -> (list Node) -> Prop :=
-  | p_start: forall g u v, eIn g u v = true -> path g u v nil
-  | p_step: forall g u v w l, 
-     path g u w l ->
-     eIn g w v = true ->
-     path g u v (w :: l) .
-
-Fixpoint path_list (g: gr a b) (u v: Node) (l: list Node) : bool :=
-  match l with
-  | nil => eIn g u v
-  | x :: tl => eIn g x v && path_list g u x tl
-  end.
-
-Lemma path_list_equiv: forall g u v l,
-  path g u v l <-> path_list g u v l = true.
-Proof.
-  intros. split; intros.
-  - induction H.
-    + simpl. assumption.
-    + simpl. rewrite andb_true_iff. split; assumption.
-  - generalize dependent v. induction l; intros; simpl.
-    + apply p_start. simpl in H. assumption.
-    + simpl in *. rewrite andb_true_iff in H. destruct H. apply p_step. apply IHl. assumption.
-      assumption.
-Qed.
-
-(*Some useful results about [path]*)
-Lemma path_app: forall g u v a l1 l2,
-  path_list g u v (l1 ++ a :: l2) = true <->
-  path_list g a v l1 = true /\ path_list g u a l2 = true.
-Proof.
-  intros. split; intros. generalize dependent v. generalize dependent l2. induction l1; intros.
-  - simpl in H. simpl. rewrite andb_true_iff in H. apply H.
-  - simpl in *. simplify'; apply IHl1 in H1; destruct H1; assumption.
-  - destruct_all. generalize dependent v. generalize dependent a0. revert l2. induction l1; intros; simpl in *;
-    simplify'.
-Qed.
-
-Lemma path_remove_cycle: forall g u v w l1 l2 l3,
-  path_list g u v (l1 ++ w :: l2 ++ w :: l3) = true ->
-  path_list g u v (l1 ++ w :: l3) = true.
-Proof.
-  intros. apply path_app in H. destruct_all. apply path_app in H0. destruct_all.
-  apply path_app. simplify'.
-Qed.
-
-(*If there is a path, then there is a path with no duplicates*)
-Lemma path_no_dups: forall g u v l,
-  path_list g u v l = true ->
-  exists l1, path_list g u v l1 = true /\ NoDup l1 /\ ~In u l1 /\  ~In v l1 /\ 
-  (forall x, In x l1 -> In x l). 
-  Proof.
-    intros. induction l using (well_founded_induction
-                       (wf_inverse_image _ nat _ (@length _)
-                          PeanoNat.Nat.lt_wf_0)).
-    destruct (NoDup_dec (N.eq_dec) l).
-    - destruct (In_dec N.eq_dec u l).
-      + eapply in_split_app_fst in i. destruct_all. clear H2. subst.
-        apply path_app in H. destruct H. specialize (H0 x). destruct H0 as [l]. 
-        rewrite app_length. simpl. assert (forall n m, n < n + S(m)) by (intros; omega). apply H0.
-        apply H. exists l. simplify'. apply N.eq_dec.
-      + destruct (In_dec N.eq_dec v l).
-        * eapply in_split_app_fst in i. destruct_all; subst. clear H2. apply path_app in H.
-          destruct H. specialize (H0 x0). destruct H0 as [l]. rewrite app_length. simpl.
-          assert (forall n m, n < m + S(n)) by (intros; omega). apply H0. apply H1. exists l.
-          simplify'. apply N.eq_dec.
-        * exists l. simplify'.
-    - rewrite no_no_dup in n. destruct_all. subst. 
-      apply path_remove_cycle in H. specialize (H0 (x0 ++ x :: x2)). destruct H0 as [l].
-      repeat(rewrite app_length; simpl). omega. apply H. exists l. simplify'. apply H5 in H4.
-      apply in_app_or in H4. destruct H4. apply in_or_app. left. apply H4. simpl in H4.
-      destruct H4. subst. solve_in. solve_in. apply N.eq_dec.
-Qed.
-
-Lemma path_implies_in_graph: forall g u v l,
-  path_list g u v l = true ->
-  vIn g u = true /\ vIn g v = true /\ (forall x, In x l -> vIn g x = true).
-Proof.
-  intros. generalize dependent v. induction l; intros; simpl in H.
-  - apply edges_valid in H. simplify'.
-  - rewrite andb_true_iff in H. destruct H. apply IHl in H0. apply edges_valid in H. crush.
-Qed. 
-
-
-(*We want a function to get the distance between two nodes. This is a horribly inefficient function to help do this*)
-(*A terrible function to find if a path of length <= n between two vertices exists*)
-Fixpoint path_of_length (g: gr a b) (u v : Node) (n: nat) {struct n} : bool :=
-  match n with
-  | 0 => eIn g u v
-  | S(m) => if eIn g u v then true else
-  fold_right (fun x t => if path_of_length g u x m && eIn g x v then true else t) false 
-  (nodeList g)
-  end.
-
-Lemma path_of_length_implies_path: forall g u v n,
-  path_of_length g u v n = true -> exists l, path_list g u v l = true /\ length l <= n.
-Proof.
-  intros. generalize dependent v. induction n; intros.
-  - simpl in H. exists nil. split. simpl. assumption. simpl. omega.
-  - simpl in H. destruct (eIn g u v) eqn : ?.
-    exists nil. split. simpl. assumption. simpl. omega.
-    assert (forall l, fold_right
-      (fun (x : Node) (t : bool) => if path_of_length g u x n && eIn g x v then true else t) false
-      l = true-> exists x, In x l /\ path_of_length g u x n = true /\ eIn g x v = true). {
-      intros. induction l; simpl in *.
-      * inversion H0.
-      * destruct (path_of_length g u a0 n && eIn g a0 v) eqn : ?.
-        -- exists a0. split. left. reflexivity. rewrite andb_true_iff in Heqb1. apply Heqb1.
-        -- apply IHl in H0. destruct H0. exists x. destruct H0. split. right. assumption.
-           apply H1. } 
-      apply H0 in H. clear H0. destruct H. destruct H. destruct H0. apply IHn in H0.
-      destruct H0. destruct H0. exists (x :: x0). split. simpl. rewrite andb_true_iff. crush. simpl. omega.
-Qed.
-
-Lemma path_of_size_implies_function: forall g u v l n,
-  length l <= n ->
-  path_list g u v l = true -> path_of_length g u v n = true.
-Proof.
-  intros. generalize dependent v. revert u. generalize dependent n. induction l; simpl in *; intros.
-  - destruct n. simpl. apply H0. simpl. rewrite H0. reflexivity.
-  - simplify. destruct n. omega. assert (length l <= n) by omega. clear H.
-    simpl. destruct (eIn g u v) eqn : ?. reflexivity.
-      assert (forall a l', In a l' ->
-      path_of_length g u a n = true ->
-      eIn g a v = true ->
-      fold_right
-  (fun (x : Node) (t : bool) => if path_of_length g u x n && eIn g x v then true else t)
-  false l' = true). { intros. induction l'; simpl in *.
-  - destruct H.
-  - destruct H. subst. rewrite H3. rewrite H2. simpl. reflexivity. apply IHl' in H. 
-    destruct (path_of_length g u a2 n && eIn g a2 v). reflexivity. apply H. }
-    apply (H a0). assert (vIn g a0 = true). { rewrite andb_true_iff in H0.
-    destruct H0. apply edges_valid in H0. apply H0. } unfold vIn in H2.
-    unfold mem in H2. destruct (in_dec N.eq_dec a0 (nodeList g)) eqn : ?. assumption.
-    rewrite Heqs in H2. inversion H2. apply IHl. apply H1. simplify'. simplify'.
-Qed.
-
-(*If there is a path, then there is a path at most as large as the number of vertices in the graph (because
-  there is a path with no duplicates and every vertex is in the graph*)
-Lemma path_shorter_than_graph_size: forall g u v l,
-  path_list g u v l = true ->
-  exists l', path_list g u v l' = true /\ length l' <= length(nodeList g).
-Proof.
-  intros. apply path_no_dups in H. destruct_all. 
-  assert (forall a, In a x -> In a (nodeList g)). intros.
-  apply path_implies_in_graph in H. destruct_all. apply H6 in H4. unfold vIn in H4.
-  unfold mem in H4. destruct (in_dec N.eq_dec a0 (nodeList g)) eqn : ?. assumption.
-  rewrite Heqs in H4. inversion H4. 
-  exists x. split. apply H. eapply NoDup_incl_length. apply H0. unfold incl. apply H4.
-Qed.
-
-(*By the above lemma, we can simply define distance by repeatedly checking if there is a list with 
-  the given distance*)
-Definition distance (g: gr a b) (u v : Node) : option nat :=
-  fold_right (fun x acc => if path_of_length g u v x then Some x else acc) None (seq 0 (natNodes g + 1)).
-
-Lemma distance_none: forall g u v,
-  distance g u v = None <-> (forall l, path_list g u v l = false).
-Proof.
-  intros.  assert (A: forall l, fold_right (fun (x : nat) (acc : option nat) => 
-    if path_of_length g u v x then Some x else acc) None l = None <->
-    (forall x, In x l -> path_of_length g u v x = false)). { intros. split; intros; induction l; simpl in *.
-    destruct H0. destruct H0. subst. destruct (path_of_length g u v x) eqn : ?. inversion H.
-    reflexivity. apply IHl. destruct (path_of_length g u v a0) eqn : ?. inversion H.
-    apply H. assumption. reflexivity. destruct (path_of_length g u v a0) eqn : ?.
-    specialize (H a0). rewrite H in Heqb0. inversion Heqb0. left. reflexivity.
-    apply IHl. intros. apply H. right. assumption. } 
-     split; intros.
-  - unfold distance in H. 
-    assert (forall x, In x (seq 0 (natNodes g + 1)) -> path_of_length g u v x = false). { intros.
-    eapply A. apply H. assumption. } clear H. clear A.
-    destruct (path_list g u v l) eqn : P.
-    + apply path_shorter_than_graph_size in P. destruct P. destruct H.
-      assert (path_of_length g u v (length x) = true). eapply path_of_size_implies_function.
-      reflexivity. assumption. 
-      assert (In (length x) (seq 0 (natNodes g + 1))). apply in_seq. split. omega. simpl.
-      assert (length (nodeList g) = natNodes g). unfold natNodes. rewrite noNodes_def. 
-      unfold nodeList. unfold ulabNodes. apply map_length. omega. 
-      apply H0 in H3. rewrite H3 in H2. inversion H2.
-    + reflexivity.
-  - unfold distance. apply A. intros. destruct (path_of_length g u v x) eqn : ?.
-    + apply path_of_length_implies_path in Heqb0. destruct Heqb0. destruct H1. rewrite H in H1.
-      inversion H1.
-    + reflexivity.
-Qed.
-
-Lemma seq_pred: forall start len h t n l,
-  seq start len = (h :: t) ++ S n :: l ->
-  In n (h :: t).
-Proof.
-  intros. generalize dependent h. revert t. revert start0. induction len; intros.
-  - simpl. simpl in H. inversion H.
-  - simpl in H. inversion H. subst. destruct t.
-    simpl in H2. simpl. destruct len. simpl in H2. inversion H2. simpl in H2. inversion H2. subst. left. reflexivity.
-    apply IHlen in H2. solve_in.
-Qed.
-
-Lemma seq_split: forall start len l1 x l2,
-  seq start len = l1 ++ x :: l2 ->
-  (forall y, In y l1 -> y < x) /\ (forall y, In y l2 -> y > x).
-Proof.
-  intros. generalize dependent start0. revert l1. revert x. revert l2. induction len; intros; simpl in H.
-  - assert (l1 = nil). destruct l1; inversion H. subst.
-    simpl in H. inversion H.
-  - destruct l1. simpl in H. inversion H. destruct l2.
-     split; intros. destruct H0. rewrite H2 in H0. destruct H0.
-     specialize (IHlen l2 n nil (S(start0))). subst. simpl in IHlen. apply IHlen in H2.
-     split; intros. destruct H0. rewrite in_seq in H0. omega.
-     inversion H; subst. specialize (IHlen l2 x l1 (S(n)) H2). split; intros. simpl in H0.
-     destruct H0. subst. assert (In x (seq (S(y)) len)). rewrite H2. solve_in. rewrite in_seq in H0.
-      omega. destruct IHlen. apply H1. assumption. apply IHlen. apply H0.
-Qed.
-
-(*This actually computes the shortest path*)
-Lemma distance_some: forall g u v n,
-  distance g u v = Some n <->
-  (exists l, path g u v l /\ length l = n) /\ (forall l, length l < n -> path_list g u v l = false).
-Proof.
-  intros. unfold distance.
-  assert (forall l, 
-  fold_right (fun (x : nat) (acc : option nat) => if path_of_length g u v x then Some x else acc) None
-  l = Some n <-> (exists l1 l2, l = l1 ++ n :: l2 /\ (forall y, In y l1 -> path_of_length g u v y = false) /\
-  path_of_length g u v n = true)). { intros. induction l; split; intros; simpl in *.
-  - inversion H.
-  - destruct_all. destruct x; inversion H.
-  - destruct (path_of_length g u v a0) eqn : ?.
-    + inversion H; subst. exists nil. exists l. split. simpl. reflexivity. split; intros.
-      destruct H0. assumption.
-    + apply IHl in H. destruct H. exists (a0 :: x). destruct_all.
-      exists x0. split. rewrite H. simpl. reflexivity.
-      split; intros. simpl in H2. destruct H2. subst. assumption. apply H0. assumption.
-      assumption.
-  - destruct_all. destruct (path_of_length g u v a0) eqn : ?. destruct x.
-    + inversion H; subst. reflexivity.
-    + simpl in H0. inversion H; subst. specialize (H0 n0). rewrite H0 in Heqb0. inversion Heqb0.
-      left. reflexivity.
-    + destruct x. inversion H; subst. rewrite Heqb0 in H1. inversion H1.
-      inversion H; subst. apply IHl. exists x. exists x0. simplify'. }
-  rewrite H. clear H. split; intros; destruct_all.
-  - apply path_of_length_implies_path in H1. split. setoid_rewrite path_list_equiv. 
-    destruct  H1. destruct H1. assert (length x1 = n \/ length x1 < n) by omega. destruct H3.
-    exists x1. split. assumption. assumption. 
-    destruct x. simpl in H. assert (natNodes g + 1 = S(natNodes g)) by omega. rewrite H4 in H.
-    simpl in H. inversion H; subst. omega. 
-    destruct n. omega. assert (length x1 <= n) by omega. 
-    apply (path_of_size_implies_function _ _ _ _ _ H4) in H1.
-    rewrite H0 in H1. inversion H1. apply seq_pred in H. apply H.
-    intros. assert (In (length l) (seq 0 (natNodes g + 1))). { rewrite in_seq.
-    assert (In n (seq 0 (natNodes g + 1))). rewrite H. solve_in. rewrite in_seq in H3.
-    omega. } rewrite H in H3. apply seq_split in H.
-    destruct H. apply in_app_or in H3. destruct H3. 
-    destruct (path_list g u v l) eqn : ?. eapply path_of_size_implies_function in Heqb0.
-    rewrite (H0 (length l)) in Heqb0. inversion Heqb0.
-    assumption. omega. reflexivity. simpl in H3. destruct H3. omega.
-    apply H4 in H3. omega.
-  - assert (n <= (natNodes g)). { assert (n <= natNodes g \/ n > natNodes g) by omega. destruct H2.
-    assumption. rewrite path_list_equiv in H. apply path_shorter_than_graph_size in H.
-    destruct H. destruct H. rewrite H0 in H. inversion H. unfold nodeList in H3.
-    unfold ulabNodes in H3. rewrite map_length in H3. rewrite <- noNodes_def in H3.
-    unfold natNodes in H2. omega. }
-    pose proof (in_split_app_fst _ (seq 0 (natNodes g + 1)) n Nat.eq_dec).
-    assert (In n (seq 0 (natNodes g + 1))). rewrite in_seq. omega.
-    apply H3 in H4. clear H3. destruct_all. exists x0. exists x1. split. assumption.
-    apply seq_split in H3. split; intros.
-    destruct H3. destruct (path_of_length g u v y) eqn : ?.
-    apply path_of_length_implies_path in Heqb0. destruct Heqb0.
-    destruct H7. rewrite H0 in H7. inversion H7. apply H3 in H5. omega. reflexivity.
-    eapply path_of_size_implies_function. assert (length x <= n) by omega. apply H5.
-    rewrite <- path_list_equiv. assumption.
-Qed. 
-
-
-(*Next step lemma 22.1 of CLRS*)
-
-End Path.
-
-End Correctness.
-
-Section Equiv.
-
-Instance need_this_for_equations : WellFounded (bf_measure_list (Node * Num.Int)).
-Proof.
-  unfold WellFounded. apply well_founded_bf_measure_list.
-Defined.
-
+(*Want to show that done is nuique*)
 Lemma match_none_size: forall g v g',
   match_ v g = (None, g') -> natNodes g = natNodes g'.
 Proof.
   intros. pose proof (match_remain_none g). erewrite H0. reflexivity. apply H.
 Qed.  
 
+Instance need_this_for_equations : WellFounded (bf_measure_list (Node * Num.Int)).
+Proof.
+  unfold WellFounded. apply well_founded_bf_measure_list.
+Defined.
+
 Equations bfs_tail (s: state) : state by wf (get_graph s, get_queue s) (bf_measure_list (Node * Num.Int)) :=
-  bfs_tail (g, nil, x, y, z) => (g, nil, x, y, z);
-  bfs_tail (g, (v, j) :: vs, d, n, t) => if (isEmpty g) then  (g, (v, j) :: vs, d, n, t) else
+  bfs_tail (g, nil, x) => (g, nil, x);
+  bfs_tail (g, (v, j) :: vs, d) => if (isEmpty g) then  (g, (v, j) :: vs, d) else
       match (match_ v g) as y return ((match_ v g = y) -> _) with
       | (Some c, g') => fun H: (match_ v g) = (Some c, g') => 
-        bfs_tail (g', (vs ++ suci c (Num.op_zp__ j (Num.fromInteger 1))), d ++ (v,j) :: nil, n + 1, M.add v (n+1) t)
-      | (None, g') => fun H: (match_ v g) = (None, g') => bfs_tail (g', vs, d, n, t)
+        bfs_tail (g', (vs ++ suci c (Num.op_zp__ j (Num.fromInteger 1))), d ++ (v,j) :: nil)
+      | (None, g') => fun H: (match_ v g) = (None, g') => bfs_tail (g', vs, d)
       end (eq_refl).
 Next Obligation.
 unfold bf_measure_list. unfold transp. apply lex1. unfold natNodes_lt. eapply match_decr_size. symmetry. apply H.
@@ -600,41 +211,32 @@ unfold bf_measure_list. unfold transp. apply lex2. unfold natNodes_eq. eapply ma
 simpl. omega.
 Defined.
 
+
 Definition expand_bfs_tail := 
-fun s : gr a b * list (Node * Num.Int) * list (Node * Num.Int) * nat * M.t nat =>
-let (p, t) := s in
-(let (p0, n) := p in
- fun t0 : M.t nat =>
- (let (p1, l) := p0 in
-  fun (n0 : nat) (t1 : M.t nat) =>
-  (let (g, l0) := p1 in
-   fun (l1 : list (Node * Num.Int)) (n1 : nat) (t2 : M.t nat) =>
-   match l0 with
-   | nil => fun (l2 : list (Node * Num.Int)) (n2 : nat) (t3 : M.t nat) => (g, nil, l2, n2, t3)
-   | p2 :: l2 =>
-       fun (l3 : list (Node * Num.Int)) (n2 : nat) (t3 : M.t nat) =>
-       (let (n3, i) := p2 in
-        fun (l4 l5 : list (Node * Num.Int)) (n4 : nat) (t4 : M.t nat) =>
-        if isEmpty g
-        then (g, (n3, i) :: l4, l5, n4, t4)
-        else
-         (let
-            (m, g') as y
-             return (match_ n3 g = y -> gr a b * list (Node * Num.Int) * list (Node * Num.Int) * nat * M.t nat) :=
-            match_ n3 g in
-          match
-            m as m0
-            return
-              (match_ n3 g = (m0, g') -> gr a b * list (Node * Num.Int) * list (Node * Num.Int) * nat * M.t nat)
-          with
-          | Some c =>
-              fun _ : match_ n3 g = (Some c, g') =>
-              bfs_tail
-                (g', l4 ++ suci c (Num.op_zp__ i (Num.fromInteger 1)), l5 ++ (n3, i) :: nil, 
-                n4 + 1, M.add n3 (n4 + 1) t4)
-          | None => fun _ : match_ n3 g = (None, g') => bfs_tail (g', l4, l5, n4, t4)
-          end) eq_refl) l2 l3 n2 t3
-   end l1 n1 t2) l n0 t1) n t0) t.
+fun s : gr a b * list (Node * Num.Int) * list (Node * Num.Int) =>
+let (p, l) := s in
+(let (g, l0) := p in
+ fun l1 : list (Node * Num.Int) =>
+ match l0 with
+ | nil => fun l2 : list (Node * Num.Int) => (g, nil, l2)
+ | p0 :: l2 =>
+     fun l3 : list (Node * Num.Int) =>
+     (let (n, i) := p0 in
+      fun l4 l5 : list (Node * Num.Int) =>
+      if isEmpty g
+      then (g, (n, i) :: l4, l5)
+      else
+       (let (m, g') as y return (match_ n g = y -> gr a b * list (Node * Num.Int) * list (Node * Num.Int)) :=
+          match_ n g in
+        match
+          m as m0 return (match_ n g = (m0, g') -> gr a b * list (Node * Num.Int) * list (Node * Num.Int))
+        with
+        | Some c =>
+            fun _ : match_ n g = (Some c, g') =>
+            bfs_tail (g', l4 ++ suci c (Num.op_zp__ i (Num.fromInteger 1)), l5 ++ (n, i) :: nil)
+        | None => fun _ : match_ n g = (None, g') => bfs_tail (g', l4, l5)
+        end) eq_refl) l2 l3
+ end l1) l.
 
 Lemma unfold_bfs_tail: forall s,
   bfs_tail s = expand_bfs_tail s.
@@ -642,12 +244,11 @@ Proof.
   intros. unfold expand_bfs_tail. apply bfs_tail_elim; intros; reflexivity.
 Qed.
 
-(*Want to prove this is valid, done and equivalent to other*)
 Lemma bfs_tail_multi: forall s,
   bfs_multi s (bfs_tail s).
 Proof.
-  intros. destruct s as [r t]. destruct r as [r n]. destruct r as [r d].
-  generalize dependent d. revert n. revert t. 
+  intros. destruct s as[r d]. 
+  generalize dependent d.
    induction (r) using (well_founded_induction (well_founded_bf_measure_list (Node * Num.Int))).
   intros.
   destruct r as [g q]. rewrite unfold_bfs_tail. simpl. destruct q eqn : Q.
@@ -665,19 +266,1840 @@ Qed.
 Lemma bfs_tail_done: forall s,
   done (bfs_tail s) = true.
 Proof.
-  intros. unfold done. destruct s as [r t]. destruct r as [r n]. destruct r as [r d].
-  generalize dependent d. revert n. revert t. 
+  intros. unfold done. destruct s as [r d].
+  generalize dependent d.  
    induction (r) using (well_founded_induction (well_founded_bf_measure_list (Node * Num.Int))).
   intros.
   destruct r as [g q]. rewrite unfold_bfs_tail. simpl. destruct q eqn : Q.
   - simpl. reflexivity.
   - destruct p. simpl. destruct (isEmpty g) eqn : G. simpl. assumption.
-    destruct (match_ n0 g) eqn : M. destruct m; simpl.
+    destruct (match_ n g) eqn : M. destruct m; simpl.
     apply H. unfold bf_measure_list. unfold transp. apply lex1. unfold natNodes_lt. eapply match_decr_size;
     symmetry; eassumption. apply H. unfold bf_measure_list. unfold transp. apply lex2.
     unfold natNodes_eq. eapply match_none_size. eassumption. unfold list_length_lt. simpl. omega.
 Qed. 
 
+End Exec.
+
+(*Proof of correctness of bfs. Later, we prove equivalence between this inductive formulation and leveln,
+  allowing us to prove the correctness of this instead*)
+Section Correctness.
+
+Definition distance := (@Path.distance a b gr Hgraph).
+
+(*As per CLRS, a None distance is equivalent to infinity*)
+Definition lt_distance (o1: option nat) (o2: option nat) :=
+  match o1, o2 with
+  | _, None => true
+  | None, _ => false
+  | Some x, Some y => leb x y
+  end.
+
+Definition plus_distance (o1: option nat) (n: nat) :=
+  match o1 with
+  | None => None
+  | Some x => Some (x + n)
+  end.
+
+(*Lemma 22.1 of CLRS*)
+Lemma distance_triangle: forall g s u v,
+  eIn g u v = true ->
+  vIn g s = true ->
+  lt_distance (distance g s v) (plus_distance (distance g s u) 1) = true.
+Proof.
+  intros. destruct (path_dec g s u).
+  - destruct e as [l]. assert ( path g s v (u :: l)). { constructor; assumption. }
+    destruct (distance g s v) eqn : D.
+    + destruct (distance g s u) eqn : D'.
+      * simpl. rewrite Nat.leb_le. unfold distance in D'. 
+        rewrite distance_some in D'. destruct D'. destruct_all; subst.
+        assert (path g u v nil). constructor. assumption.
+        unfold distance in D. rewrite distance_some in D. destruct D. destruct_all; subst; omega.
+        destruct_all. simpl. assert (n > 1 \/ n <= 1) by omega. destruct H9. rewrite path_list_equiv in H3. rewrite H7 in H3. inversion H3.
+        simpl. omega. assumption.
+        destruct_all. unfold distance in D. rewrite distance_some in D. destruct D. destruct_all. subst.
+        omega. destruct_all.  
+        assert (n<= n0 + 1 \/ n > n0 + 1) by omega. destruct H13. assumption.
+        rewrite path_list_equiv in H5.
+        assert (length l >= n0 - 1). assert (length l >= n0 - 1 \/ length l < n0 - 1) by omega.
+        destruct H14. assumption. rewrite path_list_equiv in H1. rewrite H6 in H1. inversion H1.
+        assumption.
+        assert (length l = n0 - 1 \/ length l > n0 - 1) by omega. destruct H15.
+        rewrite path_list_equiv in H2. 
+        rewrite H11 in H2. inversion H2. simpl. omega.
+        assert (path g s v (u :: x)). constructor. rewrite path_list_equiv. assumption. assumption. 
+        rewrite path_list_equiv in H16. 
+        rewrite H11 in H16. inversion H16. simpl. omega.
+      * simpl. reflexivity.
+    + simpl. unfold distance in D. rewrite distance_none in D.
+      rewrite path_list_equiv in H2. destruct D. rewrite H3 in H2. inversion H2.
+  - destruct (N.eq_dec s u). subst. unfold distance at 2. unfold Path.distance. destruct (N.eq_dec u u).
+    simpl. destruct (distance g u v) eqn : ?. unfold distance in Heqo. rewrite distance_some in Heqo.
+    destruct Heqo; destruct_all; subst. reflexivity. 
+    assert (path_list g u v nil = true). simpl. assumption. assert (n0 - 1 = 0 \/ n0 - 1 > 0) by omega.
+    destruct H7. assert (n0 = 0 \/ n0 = 1) by omega. destruct H8; subst; reflexivity.
+    rewrite H4 in H6. inversion H6. simpl. omega. unfold distance in Heqo. rewrite distance_none in Heqo.
+    destruct Heqo. specialize (H1 nil). simpl in H1. rewrite H1 in H. inversion H. contradiction.
+    assert (distance g s u = None). { unfold distance. rewrite distance_none. split. intros. 
+    destruct (path_list g s u l) eqn : ?. exfalso. apply n. exists l; rewrite path_list_equiv; assumption.
+    reflexivity. assumption. } rewrite H1. simpl. destruct (distance g s v) eqn : D'; reflexivity.
+Qed.
+
+(*We want to be able to reason about discovered and undiscovered vertices*)
+(*
+Lemma og_graph_constant: forall s s',
+  bfs_multi s s' ->
+  get_og_graph s = get_og_graph s'.
+Proof.
+  intros. induction H.
+  - reflexivity.
+  - inversion H; subst; simpl in *. assumption. assumption.
+Qed.*)
+
+Definition white (s: state) (v: Node) : bool :=
+  vIn (get_graph s) v.
+
+Definition gray (s: state) (v: Node) : bool :=
+  if In_dec N.eq_dec v (map fst (get_queue s)) then vIn (get_graph s) v else false.
+
+Definition black (s: state) (g: gr a b) (v: Node) : bool :=
+  vIn g v && negb (vIn (get_graph s) v).
+
+(*Prove correctness of colors*)
+
+(*Once a vertex is removed from the graph, it is never there again*)
+Lemma not_white_remains: forall s v s',
+  white s v = false ->
+  bfs_multi s s' ->
+  white s' v = false.
+Proof.
+  intros. unfold white in *. induction H0; simpl.
+  - assumption.
+  - inversion H0; subst; simpl in *. apply IHmulti. apply match_remain_some in H3.
+    destruct H3. destruct (vIn g' v) eqn : E. rewrite H3 in E. destruct E. rewrite H5 in H. inversion H.
+    reflexivity. apply IHmulti. apply match_remain_none in H3. subst. assumption.
+Qed.
+
+(*Each vertex appears at most once in the output*)
+
+(*TODO: Move these to helper*)
+Lemma In_InA_equiv: forall A (x : A) l,
+    In x l <-> InA eq x l.
+  Proof.
+    intros. induction l.
+    - simpl. split; intros. 
+      + destruct H.
+      + apply InA_nil in H. destruct H.
+    - simpl. split; intros.
+      + apply InA_cons. destruct H. left. subst. reflexivity. right. apply IHl. assumption.
+      + apply InA_cons in H. destruct H. left. subst. reflexivity. right. apply IHl. assumption.
+  Qed.
+
+Lemma NoDup_NoDupA: forall {a} (l: list a),
+  NoDup l <-> NoDupA eq l.
+Proof.
+  intros; split; intros; induction H; try(constructor).
+  - rewrite <- In_InA_equiv. assumption.
+  - assumption.
+  - rewrite In_InA_equiv. assumption.
+  - assumption.
+Qed.
+
+Lemma graph_subset: forall s v g,
+  valid s g v ->
+  (forall v, vIn (get_graph s) v = true -> vIn g v = true) /\
+  (forall u v, eIn (get_graph s) u v = true -> eIn g u v = true).
+Proof.
+  intros. induction H; simpl.
+  - split; intros; assumption.
+  - inversion H0; subst; simpl in *. assert (M:=H2). apply match_remain_some in H2.
+    destruct H2. split. intros. rewrite H2 in H4. apply IHvalid. apply H4.
+    intros. rewrite H3 in H4. apply IHvalid. apply H4. apply match_remain_none in H2.
+    subst. apply IHvalid.
+Qed.
+
+Lemma black_iff_dists: forall s v v' g,
+  valid s g v ->
+  black s g v' = true <-> In v' (map fst (get_dists s)).
+Proof.
+  intros. unfold black. induction H; simpl.
+  - split; intros.
+    + rewrite andb_true_iff in H0. destruct H0. rewrite H0 in H1. inversion H1.
+    + destruct H0.
+  - rewrite andb_true_iff in *. inversion H0; subst; simpl in *. split; intros.
+    + destruct (N.eq_dec v' v0).
+      * subst. rewrite in_map_iff. exists (v0, j). split; simpl; try(reflexivity).
+        solve_in.
+      * destruct H3. assert (negb (vIn g0 v') = true). { destruct (vIn g0 v') eqn : I.
+        rewrite negb_true_iff in H4. apply match_remain_some in H2.
+        destruct H2. specialize (H2 v'). destruct H2. rewrite H6 in H4. inversion H4.
+        
+         simplify'. reflexivity. } assert (In v' (map fst d)). apply IHvalid.
+        simplify'. rewrite in_map_iff in H6. destruct H6. rewrite in_map_iff.
+        exists x. split; try(simplify'); try(solve_in).
+    + rewrite in_map_iff in H3. destruct_all. apply in_app_or in H4. destruct H4.
+      assert (In v' (map fst d)). rewrite in_map_iff. exists x. simplify'.
+      rewrite <- IHvalid in H5. destruct_all. split; try(assumption). destruct (N.eq_dec v' v0).
+      subst. destruct x; simpl in *. 
+      destruct (vIn g' n) eqn : V. apply match_remain_some in H2.
+      destruct H2. rewrite H2 in V.  simplify'. reflexivity.
+      destruct (vIn g' v') eqn : I. apply match_remain_some in H2. destruct H2. rewrite H2 in I.
+      destruct I. rewrite H8 in H6. inversion H6. reflexivity. simpl in H4. destruct H4.
+      subst. simpl in *. assert (A:=H2).
+      assert (vIn g0 v0 = true). { erewrite <- match_in. exists c. exists g'. assumption. }
+      apply match_remain_some in H2. destruct H2.
+      split. pose proof (graph_subset (g0, (v0, j) :: vs, d) v); simpl in *.
+      apply H5. assumption. assumption. destruct (vIn g' v0) eqn : E.
+      rewrite H2 in E. destruct E. contradiction. reflexivity. destruct H4.
+    + apply match_remain_none in H2. subst. assumption.
+Qed.
+
+Lemma no_dups_output: forall s g v,
+  valid s g v ->
+  NoDup (map fst (get_dists s)).
+Proof.
+  intros. induction H; simpl.
+  - constructor.
+  - inversion H0; subst; simpl in *.
+    rewrite map_app. simpl. assert (map fst d ++ v0 :: nil = rev (v0 :: rev ((map fst d)))).
+    simpl. rewrite rev_involutive. reflexivity.
+    rewrite H3. rewrite NoDup_NoDupA. apply NoDupA_rev. apply eq_equivalence.
+    constructor. intro. rewrite <- In_InA_equiv in H4. rewrite <- in_rev in H4.
+    pose proof (black_iff_dists (g0, (v0, j) :: vs, d) v v0 g H) as D; unfold black in D; simpl in *.
+    apply D in H4. rewrite andb_true_iff in H4. destruct H4.
+    assert (vIn g0 v0 = true). apply match_in. exists c. exists g'. assumption.
+    rewrite H6 in H5. inversion H5. apply NoDupA_rev. apply eq_equivalence. rewrite <- NoDup_NoDupA.
+    assumption. assumption.
+Qed.
+
+Lemma color_total: forall s g v v',
+  valid s g v ->
+  vIn g v' = true ->
+  (white s v' = true \/ gray s v' = true \/ black s g v' = true).
+Proof.
+  intros. induction H.
+  - unfold start in H0. simpl in H0. unfold white; unfold gray; unfold black; simpl. left. assumption.
+  - inversion H1; subst; simpl in *.
+    + unfold white in *; unfold gray in *; unfold black in *; simpl in *.
+      destruct (N.eq_dec v' v0). subst. right. right. rewrite andb_true_iff.
+      split; try(assumption). apply match_remain_some in H3.
+      destruct H3. destruct (vIn g' v0) eqn : E.
+      rewrite H3 in E. destruct E. contradiction. reflexivity. 
+      apply IHvalid in H0. clear IHvalid. destruct H0.
+      left. apply match_remain_some in H3. destruct H3. rewrite H3. split; assumption.
+      destruct H0. destruct (N.eq_dec v0 v'). subst. contradiction.
+      destruct (in_dec N.eq_dec v' (map fst vs)).
+      right. left. destruct (in_dec N.eq_dec v' (map fst (vs ++ suci c (j + 1)%Z))).
+      apply match_remain_some in H3. destruct H3. rewrite H3. split; assumption.
+      exfalso. apply n1. rewrite in_map_iff. rewrite in_map_iff in i. destruct i. exists x. 
+      destruct H4; split; solve_in. inversion H0. rewrite andb_true_iff in H0. destruct H0.
+      right. right. rewrite andb_true_iff. split; try(assumption).
+      apply match_remain_some in H3. destruct H3. destruct (vIn g' v') eqn : V.
+      rewrite H3 in V. destruct V. rewrite H6 in H4. inversion H4. reflexivity.
+    + assert (A:=H3). apply match_remain_none in H3. subst. unfold white in *; unfold black in *; unfold gray in *; simpl in *.
+      apply IHvalid in H0. clear IHvalid. destruct H0. left. assumption.
+      destruct (N.eq_dec v0 v'). subst. destruct H0. left. assumption.
+      right. right. assumption. destruct (in_dec N.eq_dec v' (map fst vs)).
+      * destruct H0. left. assumption. right. right. assumption.
+      * destruct H0. inversion H0. right. right. assumption.
+Qed.
+
+(*Stuff about the times*)
+(*
+Lemma time_iff_done: forall s v v',
+  valid s v ->
+  (exists n, M.find v' (get_times s) = Some n) <-> black s v' = true.
+Proof.
+  intros. induction H; split; intros; unfold black in *; simpl.
+  - unfold start in H0; simpl in H0. destruct H0. rewrite F.empty_o in H0. inversion H0.
+  - unfold start in *; simpl in *. rewrite andb_true_iff in H0. destruct H0.
+    rewrite H0 in H1. inversion H1.
+  - inversion H0; subst; simpl in *.
+    + destruct (N.eq_dec v' v0).
+      * subst. rewrite andb_true_iff. split.
+        pose proof (graph_subset ((g, (v0, j) :: vs, d, n, t, g_og)) v H); simpl in *.
+        apply H4. apply match_in. exists c. exists g'. assumption.
+        apply match_remain_some in H3. destruct H3. destruct (vIn g' v0) eqn : E.
+        rewrite H3 in E. destruct E. contradiction. reflexivity.
+      * rewrite F.add_neq_o in H1. rewrite IHvalid in H1. rewrite andb_true_iff in *.
+        split. apply H1. destruct (vIn g' v') eqn : V.
+        apply match_remain_some in H3. destruct H3. rewrite H3 in V.
+        destruct V. rewrite H5 in H1. inversion H1. inversion H8.
+        reflexivity. auto.
+    + apply match_remain_none in H3. subst. apply IHvalid. assumption.
+  - inversion H0; subst; simpl in *. destruct (N.eq_dec v' v0).
+    + subst. rewrite F.add_eq_o. exists (n+1). reflexivity. reflexivity.
+    + rewrite F.add_neq_o. 
+      assert (exists n : nat, M.find (elt:=nat) v' t = Some n). apply IHvalid.
+      rewrite andb_true_iff in *. split. apply H1. destruct (vIn g v') eqn : V.
+      apply match_remain_some in H3. destruct H3. destruct H1. destruct (vIn g' v') eqn : V'.
+      inversion H5. specialize (H3 v'). destruct H3. rewrite H6 in V'.
+      inversion V'. intuition. reflexivity. apply H4. auto.
+    + apply match_remain_none in H3. subst. apply IHvalid. assumption.
+Qed. 
+*)
+
+Lemma zip_in: forall {a} {b} (l1 : list a) (l2: list b),
+  (forall x y, In (x,y) (List.zip l1 l2) -> In x l1 /\ In y l2).
+Proof.
+  intros. generalize dependent l2. induction l1; intros.
+  - simpl in H. destruct H.
+  - simpl in H. destruct l2. destruct H.
+    simpl in H.  destruct H. inversion H; subst.
+    split; simpl; left; reflexivity. simpl. apply IHl1 in H. destruct H.
+    split; right; assumption. 
+Qed. 
+
+Fixpoint replicate_nat {a} (n: nat) (x: a) :=
+  match n with
+  | O => nil
+  | S m => x :: replicate_nat m x
+  end.
+
+Definition replicate {a} (n: Z) (x: a) :=
+  replicate_nat (Z.to_nat n) x.
+
+(*TODO: See about this and how replciate is defined*)
+Axiom replicate_def: forall {a} (n: Z) (x : a),
+  replicate n x = List.replicate n x.
+
+Lemma replicate_const: forall {a} (x: a) (n: Z),
+  length (List.replicate n x) = Z.to_nat n /\ forall y, In y (List.replicate n x) -> y = x.
+Proof.
+  intros. rewrite <- replicate_def. unfold replicate. induction (Z.to_nat n); simpl.
+  - split. reflexivity. intros. destruct H.
+  - destruct IHn0. split. rewrite H. reflexivity. intros. destruct H1. subst. reflexivity.
+    apply H0. assumption.
+Qed. 
+
+Lemma filter_equiv: forall {a} (l: list a) p,
+  List.filter p l = filter p l.
+Proof.
+  intros. induction l; simpl. reflexivity. rewrite IHl. reflexivity.
+Qed.
+
+Lemma context4l'_def: forall (g: gr a b) v i x l o g' y,
+  match_ v g = (Some (i, x, l, o), g') ->
+  In y (map snd (context4l' (i, x, l, o))) <-> eIn g v y = true.
+Proof.
+  intros. unfold context4l'. split; intros.
+  - rewrite in_map_iff in H0. destruct H0. destruct x0. simpl in *. destruct H0. subst.
+    apply in_app_or in H1. destruct H1. apply match_context in H.
+    destruct_all. subst. apply H2. rewrite in_map_iff. exists (b0, y). split; auto.
+    unfold Base.op_z2218U__ in H0. unfold Base.op_zeze__ in H0. unfold Base.Eq_Char___ in H0.
+    unfold Base.op_zeze____  in H0. rewrite filter_equiv in H0. apply filter_In in H0.
+    destruct H0. apply match_context in H. destruct_all. subst. 
+    simpl in H1. rewrite N.eqb_eq in H1. subst. apply H2. rewrite in_map_iff. exists (b0, x).
+    split. reflexivity. assumption.
+  - apply match_context in H. destruct_all. subst.
+    apply H2 in H0. rewrite in_map_iff in H0. destruct H0. rewrite in_map_iff. exists x0.
+    split. apply H. destruct H. solve_in.
+Qed.
+
+Lemma snd_equiv: @Tuple.snd = @snd.
+Proof.
+  unfold Tuple.snd. unfold snd. reflexivity.
+Qed.
+
+Lemma len_acc_def: forall {a} (l : list a ) n,
+  List.lenAcc l n = (n + Z.of_nat (length l))%Z.
+Proof.
+  intros. revert n. induction l; intros; simpl.
+  - omega.
+  - rewrite IHl. rewrite Zpos_P_of_succ_nat. omega.
+Qed. 
+
+Lemma length_equiv: forall {a} (l: list a),
+  length l = Z.to_nat (List.length l).
+Proof.
+  intros. induction l; simpl.
+  - reflexivity.
+  - unfold List.length. simpl. unfold List.length in IHl. rewrite len_acc_def. 
+    rewrite len_acc_def in IHl. simpl in IHl.
+    rewrite Z2Nat.inj_add. simpl. omega. omega. omega.
+Qed.
+
+(*Need specialized lemma for zip with replicate*)
+Lemma zip_replicate: forall {a} {b} (l : list a) (m : b) x (n: b) ,
+  In (x,n) (List.zip l (List.replicate (List.length l) m)) <-> In x l /\ n = m.
+Proof.
+  intros. rewrite <- replicate_def. unfold replicate. rewrite <- length_equiv. induction l; simpl; split; intros.
+  - destruct H.
+  - destruct_all. destruct H.
+  - destruct H. inversion H; subst. split; try(left); reflexivity.
+    apply IHl in H. destruct H. subst. split. right. assumption. reflexivity.
+  - destruct H. subst. destruct H. inversion H. left. reflexivity.
+    right. apply IHl. split; try(assumption); reflexivity.
+Qed.
+
+Lemma suci_def: forall x y n (c: Context a b) v g g',
+  match_ v g = (Some c, g') ->
+  In (x,y) (suci c n) <-> y = n /\ eIn g v x = true. 
+Proof. 
+  intros. split. intros. split. unfold suci in H0. apply zip_in in H0. destruct H0. apply replicate_const in H1. assumption.
+  unfold suci in H0. apply zip_in in H0. destruct H0. unfold suc' in H0.
+  unfold Base.op_z2218U__ in H0. unfold Base.map in H0. rewrite snd_equiv in H0. 
+  destruct c. destruct p. destruct p.
+  eapply context4l'_def. apply H. apply H0.
+  intros. unfold suci. destruct H0. subst.
+  epose proof (zip_replicate (suc' c) n x n). apply H0. split.
+  unfold suc'. unfold Base.op_z2218U__. rewrite snd_equiv. unfold Base.map.
+  destruct c. destruct p. destruct p. rewrite context4l'_def. apply H1. apply H. reflexivity.
+Qed.
+
+Lemma dist_geq_0: forall s g v v' d,
+  valid s g v ->
+  In (v', d) (get_queue s) ->
+  (d >= 0)%Z.
+Proof.
+  intros. generalize dependent v'. generalize dependent d. induction H; intros.
+  - unfold start in H0; simpl in *. destruct H0. inversion H0; subst. omega. destruct H0.
+  - inversion H0; subst; simpl in *.
+    +  apply in_app_or in H1. destruct H1. eapply IHvalid. right. apply H1.
+      eapply (suci_def _ _ _ _ _ _ _ H3) in H1. destruct H1. 
+       assert ((j >=0)%Z). eapply IHvalid. left. reflexivity. omega.
+     + eapply IHvalid. right. apply H1.
+Qed. 
+
+Lemma dists_geq_0: forall s g v v' d,
+  valid s g v ->
+  In (v', d) (get_dists s) ->
+  (0 <= d)%Z.
+Proof.
+  intros. induction H.
+  - unfold start in *. simpl in *. destruct H0.
+  - inversion H1; subst; simpl in *.
+    + apply in_app_or in H0. destruct H0. apply IHvalid; assumption. simpl in H0. destruct H0.
+      inversion H0; subst.
+      pose proof (dist_geq_0 (g0, (v', d) :: vs, d0) g v v' d H). simpl in H4.
+      assert (d >= 0)%Z. apply H4. left. reflexivity. omega. destruct H0.
+    + apply IHvalid; assumption.
+Qed.
+
+Lemma queue_has_pred: forall s g v v' d,
+  valid s g v ->
+  v <> v' ->
+  In (v', (d + 1)%Z) (get_queue s) ->
+  (exists u, In (u, d) (get_dists s) /\ eIn g u v' = true).
+Proof.
+  intros. generalize dependent d. induction H; intros.
+  - unfold start in H1; simpl in H1. destruct H1. inversion H1. subst. contradiction. destruct H1.
+  - specialize (IHvalid H0). inversion H1; subst; simpl in *.
+    + apply in_app_or in H2. destruct H2.
+      * assert (exists u : Node, In (u, d) d0 /\ eIn g u v' = true). apply IHvalid.
+        right. assumption. destruct H5. destruct H5. exists x. split.
+        solve_in. assumption.
+      * apply (suci_def _ _ _ _ _ _ _ H4) in H2. destruct H2.
+        assert (d = j) by omega. subst. exists v0. split. apply in_or_app.
+        right. left. reflexivity. pose proof (graph_subset (g0, (v0, j) :: vs, d0) v g H).
+        simpl in H6; destruct H6. apply H7. assumption.
+    + apply IHvalid. right. assumption.
+Qed.
+
+Lemma finished_has_pred: forall s g v v' d,
+  valid s g v ->
+  v <> v' ->
+  In (v', (d + 1)%Z) (get_dists s) ->
+  (exists u, In (u, d) (get_dists s) /\ eIn g u v' = true).
+Proof.
+  intros. induction H.
+  - unfold start in *; simpl in *. destruct H1.
+  - inversion H2; subst; simpl in *.
+    + apply in_app_or in H1. destruct H1. apply (IHvalid H0) in H1.
+      destruct H1. exists x. split. destruct H1. solve_in. apply H1.
+      simpl in H1. destruct H1. inversion H1. 
+      subst. pose proof (queue_has_pred (g0, (v', (d + 1)%Z) :: vs, d0) g v v' d H H0).
+      simpl in H5. assert (exists u : Node, In (u, d) d0 /\ eIn g u v' = true). apply H5. left.
+      reflexivity. clear H5. destruct H6. exists x. destruct H5. split. solve_in. assumption.
+      destruct H1.
+    + apply IHvalid. assumption. assumption.
+Qed.
+
+Lemma source_in_gr: forall s g v,
+  valid s g v ->
+  vIn g v = true.
+Proof.
+  intros. induction H; simpl.
+  - assumption.
+  - inversion H0; subst; simpl in *; assumption.
+Qed.
+
+(** ** Lemma 22.2 of CLRS **)
+
+(*First, the necessary statement for queues: if (v', d) is in the queue, then d(v') >= d*)
+Lemma queue_upper_bound: forall s g v v' d,
+  valid s g v ->
+  In (v', d) (get_queue s) ->
+  lt_distance (distance g v v')  (Some (Z.to_nat d)) = true.
+Proof.
+  intros. generalize dependent v'. generalize dependent d. induction H; intros.
+  - unfold start in *; simpl in *. destruct H0. inversion H0; subst.
+    simpl. unfold distance. unfold Path.distance. destruct (N.eq_dec v' v'). reflexivity. contradiction.
+    destruct H0. 
+  - inversion H0; subst; simpl in *.
+    + apply in_app_or in H1. destruct H1. apply IHvalid. right. assumption.
+      apply (suci_def _ _ _ _ _ _ _ H3) in H1. destruct H1. subst.
+      pose proof (source_in_gr (g0, (v0, j) :: vs, d0) g v H). simpl in H1.
+      pose proof (graph_subset (g0, (v0, j) :: vs, d0) v g H). simpl in H5.
+      destruct H5. apply H6 in H4. 
+      pose proof (distance_triangle _ _ _ _ H4 H1).
+      assert (lt_distance (distance g v v0) (Some (Z.to_nat j)) = true). apply IHvalid. left.
+      reflexivity. destruct (distance g v v0) eqn : ?; simpl in *.
+      destruct (distance g v v') eqn : ?. simpl in *. rewrite Nat.leb_le in *.
+      assert ((j >= 0)%Z). eapply dist_geq_0. apply H. simpl. left. reflexivity.
+      assert (Z.to_nat j + 1 = Z.to_nat (j + 1)). assert (Z.to_nat j + Z.to_nat (1%Z) = Z.to_nat (j + 1)).
+      rewrite <- Z2Nat.inj_add. reflexivity. omega. omega. 
+      assert (Z.to_nat 1 = 1). unfold Z.to_nat. unfold Pos.to_nat. simpl. reflexivity.
+      rewrite H11 in H10. omega. omega. simpl. simpl in H7. inversion H7.
+      inversion H8.
+    + apply IHvalid. right. assumption.
+Qed. 
+
+(*Lemma 22.2 of CLRS*)
+Lemma dist_upper_bound: forall s g v v' d,
+  valid s g v ->
+  In (v', d) (get_dists s) ->
+  lt_distance (distance g v v') (Some (Z.to_nat d))  = true.
+Proof.
+  intros. induction H; simpl.
+  - unfold start in H0; simpl in H0. destruct H0.
+  - inversion H1; subst; simpl in *.
+    + apply in_app_or in H0. destruct H0. specialize (IHvalid H0).
+      apply IHvalid. simpl in H0. destruct H0. inversion H0; subst.
+      pose proof (queue_upper_bound _ _ _ v' d H). simpl in H4.
+      unfold lt_distance in H4. apply H4. left. reflexivity. destruct H0.
+    + apply IHvalid. assumption.
+Qed.
+
+Lemma map_snd_zip: forall {a b} (l1: list a) (l2: list b),
+  length l1 = length l2 ->
+  map snd (List.zip l1 l2) = l2.
+Proof.
+  intros. generalize dependent l2. induction l1; intros; simpl.
+  - simpl in H. destruct l2; try(reflexivity). simpl in H. omega.
+  - simpl in H. destruct l2. simpl in H. omega. simpl in H. inversion H.
+    simpl. rewrite IHl1. reflexivity. assumption.
+Qed.
+
+Lemma in_replicate_nat: forall {a} x (c : a) n,
+  In x (replicate_nat n c) -> x = c.
+Proof.
+  intros. induction n; simpl in *. destruct H. destruct H. subst. reflexivity. apply IHn.
+  assumption.
+Qed.
+
+Lemma replicate_sorted: forall c n,
+  Sorted Z.le (replicate n c). 
+Proof.
+  intros. unfold replicate.
+  induction (Z.to_nat n); simpl; try(constructor).
+  - assumption.
+  - apply In_InfA. intros. apply in_replicate_nat in H. subst. omega.
+Qed. 
+
+
+(** Lemma 22.3 of CLRS **)
+Lemma queue_structure: forall s g v v' d tl,
+  valid s g v ->
+  get_queue s = (v', d) :: tl ->
+  (Sorted Z.le (map snd (get_queue s))) /\ (forall v' d', In (v', d') (get_queue s) -> (d' <= d + 1)%Z).
+Proof.
+  intros. generalize dependent v'. revert d. revert tl. induction H; intros; simpl.
+  - unfold start; simpl in *. inversion H0; subst. split. constructor. constructor. constructor.
+    intros. destruct H1. inversion H1. subst. omega. destruct H1.
+  - inversion H0; subst; simpl in *.
+    + split. rewrite map_app. eapply SortA_app. apply eq_equivalence.
+      assert (Sorted Z.le (j :: map snd vs)). { specialize (IHvalid vs j v0).
+      apply IHvalid. reflexivity. } inversion H4; subst. assumption.
+      unfold suci. rewrite map_snd_zip. rewrite <- replicate_def . apply replicate_sorted.
+       pose proof (replicate_const (j+1)%Z (List.length (suc' c)) ).
+      destruct H4. rewrite  H4. rewrite length_equiv. reflexivity. intros.
+      unfold suci in H5. rewrite map_snd_zip in H5. 
+      rewrite <- In_InA_equiv in H5. rewrite <- replicate_def in H5.
+      unfold replicate in H5. apply in_replicate_nat in H5. subst.
+      rewrite <- In_InA_equiv in H4. rewrite in_map_iff in H4.
+      destruct H4. destruct H4. destruct x0; subst.
+      simpl. specialize (IHvalid vs j v0). destruct IHvalid. reflexivity.
+      specialize (H6 n i). apply H6. right. assumption.
+      epose proof (replicate_const (j + 1)%Z (List.length (suc' c))).
+      destruct H6. rewrite H6. apply length_equiv.
+      intros. apply in_app_or in H4.
+      (*d is in vs or suci *)
+      destruct vs. simpl in H1. destruct H4. simpl in H4. destruct H4.
+      unfold suci in H4. apply zip_in in H4. destruct H4.
+      rewrite <- replicate_def in H5. unfold replicate in H5.
+      apply in_replicate_nat in H5. subst.
+      assert (In (v', d) (suci c (j+1)%Z)). rewrite H1. solve_in.
+      unfold suci in H5. apply zip_in in H5. destruct H5.
+      rewrite <- replicate_def in H6. unfold replicate in H6.
+      apply in_replicate_nat in H6. subst. omega. 
+      (*other case*)
+      simpl in H1. inversion H1. subst.
+      specialize (IHvalid ((v', d) :: vs) j v0). destruct IHvalid.
+      reflexivity. inversion H5. subst.
+      inversion H10. subst. 
+      destruct H4.
+      simpl in H4. destruct H4. inversion H4. subst. omega.
+      assert (d' <= j + 1)%Z. eapply H6. right. right. apply H4.
+      omega.
+      unfold suci in H4. apply zip_in in H4. destruct H4.
+      rewrite <- replicate_def in H7. unfold replicate in H7.
+      apply in_replicate_nat in H7. subst. omega.
+    + specialize (IHvalid vs j v0). destruct IHvalid. reflexivity.
+      split. inversion H4. assumption. intros. rewrite H1 in H6.
+      destruct H6. inversion H6; subst. omega.
+      inversion H4; subst. inversion H10; subst.
+      assert (d' <= j + 1)%Z. eapply H5. right. right. apply H6. omega.
+Qed. 
+
+
+
+
+
+Lemma measure_step: forall s s',
+  bfs_step s s' ->
+  bf_measure_list (Node * Num.Int) (get_graph s', get_queue s') (get_graph s, get_queue s) .
+Proof.
+  intros. unfold bf_measure_list. unfold transp. inversion H; subst; simpl in *.
+  - apply lex1. unfold natNodes_lt. eapply match_decr_size. symmetry. apply H1.
+  - apply lex2. unfold natNodes_eq. eapply match_none_size. apply H1.  unfold list_length_lt.
+simpl. omega.
+Qed.
+
+Lemma measure_trans: forall {a} x y z,
+  bf_measure_list a x y ->
+  bf_measure_list a y z ->
+  bf_measure_list a x z.
+Proof.
+  intros. unfold bf_measure_list in *. unfold transp in *.
+  inversion H; subst.
+  - inversion H0; subst.
+    + apply lex1. unfold natNodes_lt in *. omega.
+    + apply lex1. unfold natNodes_lt in *. unfold natNodes_eq in H5. omega.
+  - inversion H0; subst.
+    + apply lex1. unfold natNodes_lt in *. unfold natNodes_eq in H1. omega.
+    + apply lex2. unfold natNodes_eq in *. omega. unfold list_length_lt in *. omega.
+Qed. 
+
+Lemma measure_antisym: forall {a} x y,
+  bf_measure_list a x y ->
+  ~bf_measure_list a y x.
+Proof.
+  intros. intro. unfold bf_measure_list in *. unfold transp in *.
+  inversion H; inversion H0; subst; unfold natNodes_lt in *; unfold natNodes_eq in *.
+  - inversion H5; subst. inversion H6; subst. omega.
+  - inversion H6; subst. inversion H7; subst. omega.
+  - inversion H6; subst. inversion H7; subst. omega.
+  - inversion H7; subst. inversion H8; subst.
+    unfold list_length_lt in *. omega.
+Qed.
+
+Lemma measure_antirefl: forall {a} x,
+  ~bf_measure_list a x x.
+Proof.
+  intros. intro. inversion H; subst; unfold transp in *; unfold natNodes_lt in *; unfold list_length_lt in *; try(omega).
+Qed.
+
+Lemma measure_multi: forall s s',
+  bfs_multi s s' ->
+  s = s' \/ bf_measure_list (Node * Num.Int) (get_graph s', get_queue s') (get_graph s, get_queue s) .
+Proof.
+  intros. induction H.
+  - left. reflexivity.
+  - destruct IHmulti. subst. right. apply measure_step. assumption.
+    right. eapply measure_trans. apply H1. apply measure_step. assumption.
+Qed.
+
+Lemma multistep_eq_measure: forall s s',
+  bfs_multi s s' ->
+  (s = s') <-> (~bf_measure_list _ (get_graph s', get_queue s') (get_graph s, get_queue s) /\
+  ~bf_measure_list (Node * Num.Int) (get_graph s, get_queue s) (get_graph s', get_queue s')). 
+Proof.
+  intros. split. intros. subst. split; intro;
+  pose proof (measure_antirefl (get_graph s', get_queue s')); contradiction. intros.
+  destruct H0. apply measure_multi in H. destruct H. subst. reflexivity. contradiction.
+Qed. 
+
+Lemma bfs_step_deterministic : forall s1 s2 s,
+  bfs_step s s1 -> bfs_step s s2 -> s1 = s2.
+Proof.
+  intros. inversion H; subst; simpl in *.
+  - inversion H0; subst; simpl in *.
+    + rewrite H10 in H2. inversion H2; subst. reflexivity.
+    + rewrite H10 in H2. inversion H2.
+  - inversion H0; subst; simpl in *.
+    + rewrite H10 in H2. inversion H2.
+    + rewrite H10 in H2. inversion H2; subst. reflexivity.
+Qed.
+
+Lemma multi_from_start: forall s s' s'',
+  bfs_multi s s'' ->
+  bfs_multi s s' ->
+  (bfs_multi s' s'' \/ bfs_multi s'' s').
+Proof.
+  intros. generalize dependent s'. induction H; intros.
+  - right. apply H0.
+  - inversion H1; subst.
+    + left. eapply multi_step. apply H. apply H0.
+    + assert (y=y0). eapply bfs_step_deterministic.
+      apply H. apply H2. subst. apply IHmulti. apply H3.
+Qed.
+
+Lemma valid_begins_with_start: forall s g v,
+  valid s g v ->
+  bfs_multi (start g v) s.
+Proof.
+  intros. induction H.
+  - constructor.
+  - eapply multi_trans. apply IHvalid.  eapply multi_step. apply H0. apply multi_refl.
+Qed.
+
+Lemma valid_multi: forall s s' g v,
+  valid s g v ->
+  valid s' g v ->
+  bfs_multi s s' \/ bfs_multi s' s.
+Proof.
+  intros. eapply multi_from_start. apply valid_begins_with_start. apply H0.
+  apply valid_begins_with_start. assumption.
+Qed.
+(*Can prove by done cannot step and bf of 1 implies not bf of other but see*)
+Lemma not_done_step: forall s g v,
+  valid s g v ->
+  (done s = false <-> exists s', bfs_step s s').
+Proof.
+  intros. split; intros.
+  - destruct s as [p d]. destruct p as [g' q].
+    unfold done in H0. simpl in H0.
+    rewrite orb_false_iff in H0. destruct H0.
+    destruct q. simpl in H0. inversion H0.
+    destruct p as [v' d'].
+    destruct (match_ v' g') eqn : M. destruct m.
+    + exists ((g0, q ++ suci c (Num.op_zp__ d' (Num.fromInteger 1)), d ++ (v', d') :: nil)).
+      constructor; assumption.
+    + exists (g0, q, d). constructor; assumption.
+  - destruct H0. unfold done in *; inversion H0; subst; simpl in *; assumption.
+Qed.
+
+(**TODO: add to helper*)
+Lemma contrapositive: forall (P Q : Prop), (P -> Q) -> (~Q -> ~P).
+Proof.
+  tauto.
+Qed. 
+
+Lemma done_cannot_step: forall s g v,
+  valid s g v ->
+  done s = true ->
+  ~(exists s', bfs_step s s').
+Proof.
+  intros. intro. pose proof (not_done_step _ _ _ H).
+  destruct H2. apply contrapositive in H3. contradiction. 
+  rewrite H0. intro. inversion H4.
+Qed.
+
+Lemma measure_done: forall s g v,
+  valid s g v ->
+  done s = true <-> (forall s', valid s' g v -> ~bf_measure_list _(get_graph s', get_queue s') (get_graph s, get_queue s)).
+Proof.
+  intros. split; intros.
+  - intro. pose proof (valid_multi _ _ _ _ H H1). destruct H3.
+    + inversion H3. subst. pose proof (measure_antirefl (get_graph s', get_queue s')).
+      contradiction. subst. pose proof (done_cannot_step _ _ _ H H0).
+      apply H6. exists y. assumption.
+    + apply measure_multi in H3. destruct H3. subst.
+      pose proof (measure_antirefl (get_graph s, get_queue s)).
+      contradiction. pose proof (measure_antisym _ _ H2). contradiction.
+  - destruct (done s) eqn : D.
+    + reflexivity.
+    + pose proof (not_done_step _ _ _ H). apply H1 in D.
+      destruct D. assert (valid x g v). eapply v_step. apply H. apply H2.
+      apply H0 in H3. apply measure_step in H2. contradiction.
+Qed.  
+
+Lemma measure_unique: forall s g v s',
+  valid s g v ->
+  valid s' g v ->
+  ~bf_measure_list _(get_graph s', get_queue s') (get_graph s, get_queue s) ->
+  ~bf_measure_list _(get_graph s, get_queue s) (get_graph s', get_queue s') ->
+  s = s'.
+Proof.
+  intros. pose proof (valid_multi _ _ _ _ H H0). destruct H3.
+  - apply measure_multi in H3. destruct H3. assumption. contradiction.
+  - apply measure_multi in H3. destruct H3. subst. reflexivity. contradiction.
+Qed. 
+
+Lemma done_unique: forall s g v s',
+  valid s g v ->
+  valid s' g v ->
+  done s = true ->
+  done s' = true ->
+  s = s'.
+Proof.
+  intros. assert (forall s', valid s' g v -> ~bf_measure_list _(get_graph s', get_queue s') (get_graph s, get_queue s)).
+  eapply measure_done. assumption. assumption.
+  assert (forall s'', valid s'' g v -> ~bf_measure_list _(get_graph s'', get_queue s'') (get_graph s', get_queue s')).
+  eapply measure_done. assumption. assumption.
+  eapply measure_unique. apply H. apply H0. apply H3. apply H0.
+  apply H4. apply H.
+Qed.
+
+(*This enables us to talk about any prior valid state, with the assurance that we will multistep to the
+  current, done state*)
+Lemma multi_done: forall s s' g v,
+  valid s g v ->
+  valid s' g v ->
+  done s = false ->
+  done s' = true ->
+  bfs_multi s s'.
+Proof.
+  intros. assert (exists s'', bfs_multi s s'' /\ done s'' = true).
+  exists (bfs_tail s). split. apply bfs_tail_multi. apply bfs_tail_done.
+  destruct H3 as [s'']. destruct H3. assert (valid s'' g v). eapply multi_valid.
+  apply H. apply H3. assert (s' = s''). eapply done_unique; try(assumption).
+  apply H0. apply H5. subst. assumption.
+Qed.
+
+(*A lemma that says that 2 states that step to each other are the closest valid states according to the well founded
+  relation*)
+Lemma bfs_step_measure_exact: forall s s' g v,
+  valid s g v ->
+  bfs_step s s' ->
+  (forall x, valid x g v -> ~ (bf_measure_list _ (get_graph x, get_queue x) (get_graph s, get_queue s) /\
+  bf_measure_list _ (get_graph s', get_queue s') (get_graph x, get_queue x))).
+Proof.
+  intros. intro. destruct H2.
+  assert (valid s' g v). eapply v_step. apply H. assumption.
+  pose proof (valid_multi _ _ _ _ H H1). destruct H5.
+  inversion H5. subst. pose proof (measure_antirefl (get_graph x, get_queue x)). contradiction.
+  subst. assert (y = s'). eapply bfs_step_deterministic. apply H6. assumption. subst.
+  eapply measure_multi in H7. destruct H7. subst. 
+  pose proof (measure_antirefl (get_graph x, get_queue x)). contradiction.
+  pose proof (measure_antisym (get_graph x, get_queue x) (get_graph s', get_queue s')).
+  apply H8 in H7. contradiction.
+  apply measure_multi in H5. destruct H5. subst.
+  pose proof (measure_antirefl (get_graph s, get_queue s)). contradiction.
+  pose proof (measure_antisym (get_graph x, get_queue x) (get_graph s, get_queue s)).
+  apply H6 in H2. contradiction.
+Qed.
+
+(*Why we needed that lemma: if s -> x and s' -> x, then s = s'*)
+Lemma valid_determ: forall s g v s' x,
+  valid s g v ->
+  valid s' g v ->
+  bfs_step s x ->
+  bfs_step s' x ->
+  s = s'.
+Proof.
+  intros. pose proof (valid_multi _ _ _ _ H H0).
+  destruct H3.
+  - apply multistep_eq_measure. apply H3.
+    apply measure_multi in H3. destruct H3. subst.
+    split; intro; pose proof (measure_antirefl (get_graph s', get_queue s')); contradiction.
+    assert (S1 := H1). assert (S2 := H2).
+    apply measure_step in H1. apply measure_step in H2. split.
+    exfalso. pose proof (bfs_step_measure_exact _ _ _ _ H S1).
+    specialize (H4 s' H0). apply H4. split; assumption.
+    intro.
+    pose proof (measure_antisym (get_graph s, get_queue s) (get_graph s', get_queue s')).
+    apply H5 in H4. contradiction.
+  - symmetry. apply multistep_eq_measure. apply H3.
+    apply measure_multi in H3. destruct H3. subst.
+    split; intro; pose proof (measure_antirefl (get_graph s, get_queue s)); contradiction.
+    assert (S1 := H1). assert (S2 := H2).
+    apply measure_step in H1. apply measure_step in H2. split.
+    exfalso. pose proof (bfs_step_measure_exact _ _ _ _ H0 S2).
+    specialize (H4 s H). apply H4. split; assumption.
+    intro.
+    pose proof (measure_antisym (get_graph s, get_queue s) (get_graph s', get_queue s')).
+    apply H5 in H3. contradiction.
+Qed.
+
+
+(*Reachability*)
+Lemma queue_reachable: forall s g v v',
+  valid s g v ->
+  In v' (map fst (get_queue s)) ->
+  v = v' \/ (exists l, path g v v' l).
+Proof.
+  intros. generalize dependent v'. induction H; intros; subst.
+  - unfold start in *; simpl in *. destruct H0. subst. left. reflexivity. destruct H0.
+  - inversion H0; subst; simpl in *.
+    + rewrite map_app in H1. apply in_app_or in H1. destruct H1.
+      apply IHvalid. right. assumption. rewrite in_map_iff in H1.
+      destruct H1. destruct x. simpl in H1. destruct H1; subst.
+      apply (suci_def _ _ _ _ _  _ _ H3) in H4. destruct H4; subst.
+      specialize (IHvalid v0). destruct IHvalid. left. reflexivity. subst.
+      right. exists nil. constructor. pose proof (graph_subset _ _ _ H).
+      destruct H1. apply H5. simpl. assumption.
+      destruct H1. right. exists (v0 :: x). constructor. assumption.
+      pose proof (graph_subset _ _ _ H).
+      apply H5. simpl. assumption.
+    + apply IHvalid. right. assumption.
+Qed. 
+
+Theorem output_is_reachable: forall s g v v',
+  valid s g v ->
+  In v' (map fst (get_dists s)) ->
+  v = v' \/ (exists l, path g v v' l).
+Proof.
+  intros. induction H; subst.
+  - unfold start in *; simpl in *. destruct H0.
+  - inversion H1; subst; simpl in *.
+    + rewrite map_app in H0. apply in_app_or in H0. destruct H0.
+      apply IHvalid. assumption. eapply queue_reachable. apply H. simpl.
+      simpl in H0. destruct H0; subst. left. reflexivity. destruct H0.
+    + apply IHvalid. assumption.
+Qed. 
+
+
+(*Now the harder side: everything that is reachable is in the output*)
+
+(*plan: prove that vertex in graph iff it is not in output *)
+Lemma graph_iff_not_output: forall s g v v',
+  valid s g v ->
+  vIn g v' = true ->
+  In v' (map fst (get_dists s)) <-> (vIn (get_graph s) v' = false).
+Proof.
+  intros. induction H; split; intros; simpl in *.
+  - destruct H1.
+  - rewrite H1 in H0. inversion H0.
+  - inversion H1; subst; simpl in *.
+    + rewrite map_app in H2. apply in_app_or in H2.
+      destruct H2. assert (vIn g0 v' = false). apply IHvalid.
+      assumption. assumption. apply match_remain_some in H4.
+      destruct H4. specialize (H4 v'). destruct H4. apply contrapositive in H4.
+      destruct (vIn g' v'). contradiction. reflexivity. intro. 
+      destruct H8. rewrite H8 in H5. inversion H5.
+      simpl in H2. destruct H2. subst. apply match_remain_some in H4.
+      destruct H4. specialize (H2 v'). destruct H2. apply contrapositive in H2.
+      destruct (vIn g' v'). contradiction. reflexivity. intro. destruct H6. contradiction.
+      destruct H2.
+    + apply match_remain_none in H4. subst. apply IHvalid. assumption. assumption.
+  - inversion H1; subst; simpl in *.
+    + destruct (N.eq_dec v' v0). subst.
+      rewrite map_app. apply in_or_app. right. simpl. left. reflexivity.
+      apply match_remain_some in H4. destruct H4. specialize (H4 v').
+      destruct H4. apply contrapositive in H6. destruct (vIn g0 v') eqn : V.
+      exfalso. apply H6. split. reflexivity. assumption. rewrite map_app.
+      apply in_or_app. left. rewrite IHvalid. reflexivity. assumption. 
+      destruct (vIn g' v'). inversion H2. auto.
+    + apply IHvalid. assumption. apply match_remain_none in H4. subst. assumption.
+Qed.
+
+Lemma output_preserved_strong: forall s v g v' s' (d : Num.Int),
+  valid s g v ->
+  bfs_multi s s' ->
+  In (v' d) (get_dists s) ->
+  In (v' d) (get_dists s').
+Proof.
+  intros. induction H0. assumption. assert (valid y g v). eapply v_step. apply H. assumption.
+  specialize (IHmulti H3). clear H3. inversion H0; subst; simpl in *; apply IHmulti; solve_in.
+Qed.
+
+Lemma output_preserved: forall s v g v' s',
+  valid s g v ->
+  bfs_multi s s' ->
+  In v' (map fst (get_dists s)) ->
+  In v' (map fst (get_dists s')).
+Proof.
+  intros. rewrite in_map_iff in *. destruct H1. exists x. destruct H1.
+  split. assumption. destruct x; simpl. subst. eapply output_preserved_strong.
+  apply H. apply H0. assumption.
+Qed.
+
+Lemma graph_subset': forall s v g s',
+  valid s g v ->
+  bfs_multi s s' ->
+  (forall v, vIn (get_graph s') v = true -> vIn (get_graph s) v = true) /\
+  (forall u v, eIn (get_graph s') u v = true -> eIn (get_graph s) u v = true).
+Proof.
+  intros. induction H0; simpl.
+  - split; intros; assumption.
+  - assert (valid y g v). eapply v_step. apply H. assumption.
+    specialize (IHmulti H2). clear H2. inversion H0; subst; simpl in *.
+    assert (M:=H3). apply match_remain_some in H3.
+    destruct H3. split. intros. destruct IHmulti. apply H6 in H5.
+    rewrite H3 in H5. destruct H5. assumption.
+    intros. destruct IHmulti. apply H7 in H5.
+    rewrite H4 in H5. destruct H5. assumption. apply match_remain_none in H3. subst. apply IHmulti.
+Qed.
+
+Lemma queue_in_graph: forall s v g v',
+  valid s g v ->
+  In v' (map fst (get_queue s)) -> 
+  vIn g v' = true.
+Proof.
+  intros. induction H.
+  - unfold start in *. simpl in *. destruct H0. subst. assumption. destruct H0.
+  - inversion H1; subst; simpl in *.
+    + rewrite map_app in H0. apply in_app_or in H0. destruct H0.
+      apply IHvalid. right. assumption. rewrite in_map_iff in H0.
+      destruct H0. destruct x. destruct H0; subst. apply (suci_def n i (j + 1)%Z) in H3.
+      rewrite H3 in H4. destruct H4. subst. simpl. 
+      apply edges_valid in H4. destruct H4.
+      pose proof (graph_subset _ _ _ H). destruct H5. apply H5. simpl. assumption.
+    + apply IHvalid. right. assumption.
+Qed.
+
+Lemma queue_added_to_output: forall s v g v' s',
+  valid s g v ->
+  bfs_multi s s' ->
+  In v' (map fst (get_queue s)) ->
+  ~In v' (map fst (get_queue s')) ->
+  In v' (map fst (get_dists s')).
+Proof.
+  intros. induction H0.
+  - contradiction.
+  - inversion H0; subst; simpl in *.
+    + destruct H1. subst. eapply output_preserved.
+      eapply v_step. apply H. apply H0. assumption. simpl. rewrite map_app.
+      apply in_or_app. right. simpl. left. reflexivity.
+      apply IHmulti. eapply v_step. apply H. assumption.
+      rewrite map_app. apply in_or_app. left. apply H1. assumption.
+    + destruct H1. subst. rewrite graph_iff_not_output. pose proof (graph_subset' _ _ _ z H).
+      destruct H1. eapply multi_step. apply H0. assumption. simpl in *. 
+      specialize (H1 v'). apply contrapositive in H1. destruct (vIn (get_graph z) v').
+      contradiction. reflexivity. 
+      destruct (vIn g0 v') eqn : M. rewrite <- match_in in M.
+      destruct M. destruct H7. rewrite H7 in H5. inversion H5. auto. 
+      eapply multi_valid. apply H. eapply multi_step. apply H0. assumption.
+      eapply queue_in_graph. apply H. simpl. left. reflexivity. 
+      apply IHmulti. eapply v_step. apply H. assumption. assumption. assumption.
+Qed.
+     
+(*An important lemma: If a vertex is on the queue at any point, when we multistep to the end, it is in
+  the list of distances*)
+Lemma queue_ends_in_output: forall s v g s' v',
+  valid s g v ->
+  bfs_multi s s' ->
+  done s' = true ->
+  In v' (map fst (get_queue s)) ->
+  In v' (map fst (get_dists s')).
+Proof.
+  intros. unfold done in H1. rewrite orb_true_iff in H1.
+  destruct H1. destruct (get_queue s') eqn : E. 
+  eapply queue_added_to_output. apply H. assumption. assumption. rewrite E. simpl. auto.
+  simpl in H1. inversion H1. rewrite graph_iff_not_output. 
+  rewrite isEmpty_def in H1. apply H1. apply v'. 
+  eapply multi_valid. apply H. assumption. eapply queue_in_graph. apply H. assumption.
+Qed.
+
+(*If a vertex is in the distances at any point, there must be a step when it was added to the distances*)
+Lemma output_is_added: forall s v g v' d,
+  valid s g v ->
+  In (v', d) (get_dists s) ->
+  (exists s' c g', valid s' g v /\ bfs_multi s' s  /\ (exists l1,
+    get_queue s' = l1 ++ suci c (Num.op_zp__ d (Num.fromInteger 1)) /\ (forall s'', valid s'' g v ->
+     bfs_step s'' s' ->
+    ~In v' (map fst (get_dists s'')) /\ (match_ v' (get_graph s'') = (Some c, g')) /\ 
+      get_queue s'' = (v', d) :: l1)) /\ s' <> start g v /\ (exists l2, get_dists s' = l2 ++ (v', d) :: nil) ).
+Proof.
+  intros. induction H.
+  - unfold start in H0. simpl in *. destruct H0.
+  - inversion H1; subst; simpl in *.
+    + assert (~In v0 (map fst d0)). assert (valid ( (g', vs ++ suci c (j + 1)%Z, d0 ++ (v0, j) :: nil)) g v).
+      eapply v_step. apply H. assumption. apply no_dups_output in H4. simpl in H4. rewrite NoDup_NoDupA in H4.
+      rewrite map_app in H4. simpl in H4. apply NoDupA_swap in H4. inversion H4; subst.
+      intro. rewrite In_InA_equiv in H5. rewrite app_nil_r in H7. contradiction.
+      apply eq_equivalence. destruct (N.eq_dec v' v0). subst. apply in_app_or in H0. destruct H0.
+      rewrite in_map_iff in H4. exfalso. apply H4. exists (v0, d). split; simpl. reflexivity. assumption.
+      simpl in H0. destruct H0. inversion H0; subst. 
+      exists (g', vs ++ suci c (d + 1)%Z, d0 ++ (v0, d) :: nil). exists c. exists g'.
+      split. eapply v_step. apply H. assumption.
+      split. apply multi_refl.
+      split. exists vs. split. reflexivity. intros.
+      assert (s'' = (g0, (v0, d) :: vs, d0)). eapply valid_determ. apply H5.
+      assumption. apply H6. assumption. subst. simpl in *. split. assumption. split.  assumption.
+      reflexivity. split.
+      unfold start. simpl. intro. inversion H5; subst. destruct d0; inversion H9.
+      exists d0. simpl. reflexivity.
+      destruct H0. apply in_app_or in H0. destruct H0.
+      apply IHvalid in H0. clear IHvalid. destruct H0 as [s']. destruct H0 as [c'].
+      destruct H0 as [g'']. destruct_all. exists s'. exists c'. exists g''. split.
+      assumption. split. eapply multi_trans. apply H5. apply multi_R. assumption.
+      split. exists x. split. assumption. split. apply H9. assumption. assumption. apply H9.
+      assumption. assumption. split. apply H7. exists x0. assumption.
+      destruct H0. inversion H0; subst.
+      contradiction. destruct H0.
+    + apply IHvalid in H0. clear IHvalid. destruct H0 as [s']. destruct H0 as [c'].
+      destruct H0 as [g'']. destruct_all. exists s'. exists c'. exists g''.
+      repeat(split; try(assumption)). eapply multi_trans. apply H4. apply multi_R. assumption.
+      exists x. split. assumption. apply H8. exists x0. assumption.
+Qed.
+
+Lemma prior_state: forall s g v,
+  valid s g v ->
+  s <> (start g v) ->
+  (exists s', valid s' g v /\ bfs_step s' s).
+Proof.
+  intros. inversion H; subst.
+  - contradiction.
+  - exists s'. split; assumption.
+Qed.
+(*
+Lemma state_eq_dec: forall s s' g v,
+  valid s g v ->
+  valid s' g v ->
+  s = s' \/ s <> s'.
+Proof.
+  intros. pose proof (valid_multi _ _ _ _ H H0). destruct H1.
+  - apply measure_multi in H1. destruct H1. left. assumption.
+    right. intro. subst. pose proof (measure_antirefl (get_graph s', get_queue s')); contradiction.
+  - apply measure_multi in H1. destruct H1. left. subst. reflexivity.
+    right. intro. subst. pose proof (measure_antirefl (get_graph s', get_queue s')); contradiction.
+Qed.
+*)
+Lemma valid_in: forall s g v,
+  valid s g v ->
+  vIn g v = true.
+Proof.
+  intros. induction H. assumption. assumption.
+Qed.
+
+(*Last lemma before reachability*)
+Lemma edge_in_state: forall s g v u' v',
+  valid s g v ->  
+  eIn g u' v' = true ->
+  eIn (get_graph s) u' v' = true <-> (vIn (get_graph s) u' = true /\ vIn (get_graph s) v' = true).
+Proof.
+  intros. induction H.
+  - unfold start; simpl. split; intros.
+    + apply edges_valid. assumption.
+    + assumption.
+  - specialize (IHvalid H0). inversion H1; subst; simpl in *.
+    + split; intros.
+      * apply edges_valid. assumption.
+      * destruct H4. apply match_remain_some in H3. destruct H3. apply H3 in H4.
+        apply H3 in H5. rewrite H6. split. rewrite IHvalid. destruct_all. split; assumption.
+        destruct_all; split; assumption.
+    + apply match_remain_none in H3. subst. apply IHvalid.
+Qed.
+
+(*plan is as follows:
+1. we know that every vertex that was finished has state it was finished
+2. so for a vertex, look at ancestor in path. Must have been seen by induction, so has state
+    it is on queue, so has state it is finished, so has state it was added to finished list
+3. In that state, if (p, c) in graph (from prior state, which exists), then in succs, so done
+4. Otherwise, by lemma below, p or c is in distance, if c is there, good, if p there contradiction
+QED
+    
+
+Lemma: if an edge (u,v) is in the graph, at any state, either (u,v) is in the current graph, or
+  u or v are in the output*)
+
+(*First, prove everything reachable is in queue at some point*)
+Lemma reachable_in_queue: forall g v v',
+  (exists l, path g v v' l) ->
+  (exists s, valid s g v /\ In v' (map fst (get_queue s))).
+Proof.
+  intros. destruct H as [l]. generalize dependent v'.
+  induction l using (well_founded_induction
+                     (wf_inverse_image _ nat _ (@length _)
+                        PeanoNat.Nat.lt_wf_0)).
+  intros. destruct l.
+  - inversion H0; subst.
+    assert (vIn g v = true). pose proof (edges_valid _ _ _ H1).
+    destruct H2. assumption. assert (V:= H2). apply match_in in H2.
+    destruct H2 as [c]. destruct H2 as [g']. 
+    exists ((g',  suci c (Num.op_zp__ 0%Z (Num.fromInteger 1)), (v, 0%Z) :: nil)).
+    split. eapply v_step. apply v_start. assumption. unfold start.
+    replace (suci c (Num.op_zp__ 0%Z (Num.fromInteger 1))) with (nil ++ suci c (Num.op_zp__ 0%Z (Num.fromInteger 1)))
+    by reflexivity. replace ((v, 0%Z) :: nil) with (nil ++ (v, 0%Z) :: nil) by (reflexivity).
+    eapply bfs_find. destruct (isEmpty g) eqn : E. rewrite isEmpty_def in E. rewrite E in V.
+    inversion V. apply v. reflexivity. apply H2. simpl. rewrite in_map_iff. 
+    exists (v', 1%Z). split. simpl. reflexivity. rewrite suci_def.
+    split. reflexivity. apply H1. apply H2.
+  - inversion H0; subst. simpl in H.
+    assert (exists s : state, valid s g v /\ In n (map fst (get_queue s))). eapply H.
+    assert (length l < S(length l)) by omega. apply H1. assumption.
+    destruct H1 as [s]. destruct H1. 
+    assert (exists sd, done sd = true /\ bfs_multi s sd). exists (bfs_tail s).
+    split. apply bfs_tail_done. apply bfs_tail_multi. destruct H3 as [sd]. destruct H3.
+    pose proof (queue_ends_in_output _ _ _ _ _ H1 H4 H3 H2).
+    assert (valid sd g v). eapply multi_valid. apply H1. assumption.
+    rewrite in_map_iff in H5. destruct H5. destruct x as [n' d]. simpl in H5. destruct H5; subst.
+    pose proof (output_is_added _ _ _ _ _ H8 H9). destruct H5 as [sp]. destruct H5 as [c].
+    destruct H5 as [g']. destruct H5. destruct H10. destruct H11. destruct H11 as [l1].
+    (*need prior state*)
+    destruct H12. destruct H13. pose proof (prior_state _ _ _ H5 H12). destruct H14 as [sb]. destruct H14.
+    pose proof (edge_in_state _ _ _ _ _ H14 H7). destruct H11 as [A H11].
+    specialize (H11 _ H14 H15). destruct H11. destruct H17. destruct (vIn (get_graph sb) v') eqn : M.
+    + assert (vIn (get_graph sb) n = true). erewrite <- match_in. exists c. exists g'. assumption.
+      rewrite H19 in H16. assert (eIn (get_graph sb) n v' = true). rewrite H16. split; reflexivity.
+      exists sp. split; try(assumption). rewrite A.  rewrite map_app. apply in_or_app. right.
+      pose proof (suci_def v' (Num.op_zp__ d (Num.fromInteger 1)) (Num.op_zp__ d (Num.fromInteger 1))
+      c n (get_graph sb) g' H17). simpl in H21. destruct H21.
+      rewrite H20 in H21. rewrite in_map_iff. exists (v', (d+1)%Z). split. reflexivity.
+      simpl. apply H22. rewrite H20. split; reflexivity.
+    + rewrite <- graph_iff_not_output in M. rewrite in_map_iff in M. destruct M. destruct x0. simpl in H19; destruct H19; subst.
+      pose proof (output_is_added _ _ _ _ _ H14 H20). destruct_all.
+      pose proof (prior_state _ _ _ H19 H23). destruct H26. exists x5. destruct H26. 
+      specialize (H25 _ H26 H27). destruct_all. split. assumption. rewrite H29. simpl.
+      left. reflexivity. apply H14. apply edges_valid in H7. destruct H7; assumption.
+Qed.
+
+(*Now, everything reachable is in the ouptut*)
+Lemma reachable_in_output: forall g v v' s,
+  valid s g v ->
+  done s = true ->
+  (exists l, path g v v' l) ->
+  In v' (map fst (get_dists s)).
+Proof.
+  intros. eapply reachable_in_queue in H1. destruct H1 as [s']. destruct H1.
+  eapply queue_ends_in_output. apply H1. destruct (done s') eqn : D.
+  assert (s = s'). eapply done_unique. apply H. apply H1. assumption. assumption.
+  subst. apply multi_refl. eapply multi_done. apply H1. apply H. assumption. assumption.
+  assumption. assumption.
+Qed.
+
+Lemma v_in_output: forall s g v,
+  valid s g v ->
+  s = start g v \/ In v (map fst (get_dists s)).
+Proof.
+  intros. induction H.
+  - left. reflexivity.
+  - inversion H0; subst; simpl in *.
+    + right. destruct (N.eq_dec v v0). subst.
+      rewrite map_app. simpl. solve_in.
+      unfold start in IHvalid. simpl in IHvalid.
+      rewrite map_app. destruct IHvalid. inversion H3; subst. contradiction.
+      solve_in.
+    + destruct IHvalid. unfold start in H3. inversion H3. subst.
+      assert (vIn g v = false). destruct (vIn g v) eqn : V.
+      rewrite <- match_in in V. destruct_all. rewrite H4 in H2. inversion H2. reflexivity.
+      assert (vIn g v = true). eapply valid_in. apply H. rewrite H5 in H4. inversion H4.
+      right. assumption.
+Qed.
+
+Lemma done_not_start: forall g v,
+  vIn g v = true ->
+  done (start g v) = false.
+Proof.
+  intros. unfold start. unfold done. simpl. destruct (isEmpty g) eqn : E.
+  rewrite isEmpty_def in E. rewrite E in H. inversion H. apply v. reflexivity.
+Qed.  
+
+(** Proof the BFS computes all reachable vertices **)
+Theorem output_iff_reachable: forall s g v v',
+  valid s g v ->
+  done s = true ->
+  In v' (map fst (get_dists s)) <-> v = v' \/ (exists l, path g v v' l).
+Proof.
+  intros. split; intros.
+  - eapply output_is_reachable. apply H. apply H1.
+  - destruct H1. subst. assert (vIn g v' = true). eapply valid_in. apply H.
+    apply v_in_output in H. destruct H. subst. rewrite done_not_start in H0. inversion H0.
+    apply H1. assumption. eapply reachable_in_output. apply H. apply H0. apply H1.
+Qed.
+   
+
+(** Correctness of BFS **)
+
+(*Find distance from state*)
+Definition find_dist s v :=
+  fold_right (fun x acc => if N.eq_dec (fst x) v then Some (Z.to_nat (snd x)) else acc) None (get_dists s).
+
+Lemma find_dist_in: forall s g v v' n,
+  valid s g v ->
+  find_dist s v' = Some n <-> In (v',(Z.of_nat n)) (get_dists s).
+Proof.
+  intros. pose proof no_dups_output _ _ _ H. unfold find_dist.
+  assert (forall l, NoDup (map fst l) ->
+   (forall n, In n (map snd l) -> (0 <= n)%Z) ->
+   fold_right (fun (x : N * Z) (acc : option nat) => if N.eq_dec (fst x) v' then Some (Z.to_nat (snd x)) else acc)
+  None l = Some n <-> In (v', Z.of_nat n) l). { intros; induction l; split; intros; simpl in *.
+  - inversion H3.
+  - destruct H3.
+  - destruct a0. simpl in *. destruct (N.eq_dec n0 v') eqn : ?. subst. inversion H3; subst.
+    left. rewrite Z2Nat.id. reflexivity. apply H2. left. reflexivity. 
+    right. apply IHl. inversion H1; assumption. intros. apply H2. right. assumption. assumption.
+  - destruct a0; simpl in *. destruct H3. inversion H3; subst. destruct (N.eq_dec v' v').
+    rewrite Nat2Z.id. reflexivity. contradiction. destruct (N.eq_dec n0 v'). subst.
+    inversion H1. subst. assert (In v' (map fst l)). rewrite in_map_iff. exists (v', Z.of_nat n).
+    split; try(reflexivity); assumption. contradiction. rewrite IHl. assumption. inversion H1; assumption.
+    intros. apply H2. right. assumption. } apply H1.
+    assumption. intros. rewrite in_map_iff in H2. destruct H2.
+    destruct x. destruct H2. simpl in H2; subst. eapply dists_geq_0. apply H.  apply H3.
+Qed.
+
+Lemma find_dist_not: forall s v,
+  find_dist s v = None <-> (forall y, ~In (v, y) (get_dists s)).
+Proof.
+  intros. unfold find_dist. assert (forall l, 
+  fold_right (fun (x : N * Z) (acc : option nat) => if N.eq_dec (fst x) v then Some (Z.to_nat (snd x)) else acc) None
+  l = None <-> (forall y : Num.Int, ~ In (v, y) l)). { intros.
+  induction l; split; intros; simpl in *.
+  - auto.
+  - reflexivity.
+  - destruct a0. simpl in *. destruct (N.eq_dec n v). inversion H.
+    intro. rewrite IHl in H. destruct H0. inversion H0; subst. contradiction.
+    apply (H y); assumption.
+  - destruct a0. simpl. destruct (N.eq_dec n v). subst. exfalso. apply (H z).
+    left. reflexivity. rewrite IHl. intros. intro. apply (H y). right. assumption. }
+    apply H.
+Qed.
+
+(*The start vertex appears with distance 0 in the output*)
+Lemma second_state: forall s g v,
+  vIn g v = true ->
+  bfs_step (start g v) s ->
+  get_dists s = (v, 0%Z) :: nil.
+Proof.
+  intros. unfold start in H0. inversion 0; subst; simpl. reflexivity.
+  rewrite <- match_in in H. destruct H. destruct H. rewrite H in H8. inversion H8.
+Qed.
+
+Lemma dists_nil_iff_start: forall s g v,
+  valid s g v ->
+  get_dists s = nil <-> s = start g v.
+Proof.
+  intros. induction H.
+  - split; intros; try(reflexivity).
+  - split; intros.
+    + inversion H0; subst; simpl in *.
+      * destruct d; inversion H1.
+      * subst. unfold start in IHvalid. destruct IHvalid.
+        specialize (H1 eq_refl). inversion H1; subst.
+        pose proof (valid_in _ _ _ H). rewrite <- match_in in H5.
+        destruct_all. rewrite H5 in H3. inversion H3.
+    + subst. inversion H0; subst; simpl in *.
+      * destruct d; inversion H5.
+      * unfold start in IHvalid. destruct IHvalid. 
+        specialize (H1 eq_refl). inversion H1; subst.
+Qed.
+
+Lemma multi_from_second: forall s g v s',
+  valid s g v  ->
+  bfs_step (start g v) s' ->
+  s = start g v \/ bfs_multi s' s.
+Proof.
+  intros. induction H.
+  - left. reflexivity.
+  - specialize (IHvalid H0). destruct IHvalid. subst.
+    assert (s = s'). eapply bfs_step_deterministic. apply H1. apply H0. subst.
+    right. apply multi_refl. right. eapply multi_trans. apply H2. eapply multi_step.
+    apply H1. apply multi_refl.
+Qed. 
+
+Lemma start_0_dist: forall s g v,
+  valid s g v ->
+  (get_dists s) <> nil ->
+  In (v, 0%Z) (get_dists s).
+Proof.
+  intros. assert (exists s', bfs_step (start g v) s').
+  assert (vIn g v = true) by (eapply valid_in; apply H).
+  pose proof (done_not_start g v H1). rewrite not_done_step in H2.
+  apply H2. apply v_start. apply H1. destruct H1 as [s'].
+  pose proof (multi_from_second _ _ _ _ H H1). destruct H2. subst.
+  rewrite dists_nil_iff_start in H0. contradiction. apply H. 
+  eapply output_preserved_strong. eapply v_step. apply v_start.
+  apply valid_in in H. apply H. apply H1. assumption.
+  erewrite second_state. simpl. left. reflexivity. 
+  apply valid_in in H. apply H. apply H1.
+Qed.
+
+Lemma NoDup_pairs: forall {a b} (l1 : list (a * b)) x y y',
+  NoDup (map fst l1) ->
+  In (x,y) l1 ->
+  In (x, y') l1 ->
+  y = y'.
+Proof.
+  intros. induction l1.
+  - destruct H0.
+  - simpl in *. destruct a1. simpl in H. inversion H. subst.
+    destruct H0. inversion H0; subst. destruct H1. inversion H1; subst.
+    reflexivity. assert (In x (map fst l1)). rewrite in_map_iff. exists (x, y').
+    simpl. split. reflexivity. assumption. contradiction.
+    destruct H1. inversion H1; subst. assert (In x (map fst l1)). rewrite in_map_iff.
+    exists (x, y). simpl. split. reflexivity. assumption. contradiction.
+    apply IHl1; assumption.
+Qed.
+
+(*If a vertex is on the queue once and not in the distances, then it multisteps
+  to a point where this value is at the front of the queue*)
+(*
+Lemma first_finish_first: forall s s' g v v' d' v'' d'' l1 l2 l3,
+  valid s g v ->
+  get_queue s = l1 ++ (v', d') :: l2 ++ (v'', d'') :: l3 ->
+  (forall x, In x (map fst l1) -> x <> v') ->
+  (forall x, In x (map fst ( l1 ++ (v', d') :: l2)) -> x <> v'') ->
+  In v' (map fst (get_dists s)) = false ->
+  In v'' (map fst (get_dists s)) = false ->
+  bfs_multi s s' ->
+  *)
+
+(*A key characterization of distances: If (v', d) is the first instance of v' on the queue and v' has not
+  yet been discovered, when we step, either (v', d) is in the output, or the same condition holds*)
+Lemma first_queue_constant: forall s g v v' d' l1 l2 s',
+  valid s g v ->
+  get_queue s = l1 ++ (v', d') :: l2 ->
+  (forall x, In x (map fst l1) -> x <> v') ->
+  ~In v' (map fst (get_dists s)) ->
+  bfs_step s s' ->
+  (In (v', d') (get_dists s') \/ 
+  (~In v' (map fst (get_dists s')) /\
+  exists l1 l2, get_queue s' = l1 ++ (v', d') :: l2  /\
+  (forall x, In x (map fst l1) -> x <> v'))).
+Proof.
+  intros. inversion H3; subst; simpl in *.
+  - destruct (N.eq_dec v0 v'). subst. left.
+    destruct l1. simpl in H0. inversion H0. subst. solve_in.
+    simpl in H0. inversion H0; subst. 
+    specialize (H1 v'). simpl in H1. 
+    assert (v' <> v') by (apply H1; left; reflexivity); contradiction.
+    destruct l1. simpl in H0. inversion H0; subst. contradiction.
+    destruct p. inversion H0; subst. right. split. intro.
+    rewrite map_app in H6. apply in_app_or in H6. destruct H6. contradiction.
+    simpl in H6. destruct H6; subst. contradiction. destruct H6.
+    exists l1. exists (l2 ++ suci c (i + 1)%Z). split. rewrite <- app_assoc.
+    simpl. reflexivity. intros. apply H1. simpl. right. assumption.
+  - assert (vIn g0 v' = true). destruct (vIn g0 v') eqn : E. reflexivity.
+     replace g0 with (get_graph (g0, (v0, j) :: vs, d)) in E by reflexivity.
+    rewrite <- graph_iff_not_output in E. simpl in E. contradiction.
+    apply H. 
+    eapply queue_in_graph. apply H. rewrite H0. simpl.
+    rewrite map_app. apply in_or_app. right. simpl. left. reflexivity.
+    right. split. assumption. destruct l1. simpl in H0. inversion H0; subst.
+    rewrite <- match_in in H6. destruct_all. rewrite H6 in H5. inversion H5.
+    inversion H0; subst. exists l1. exists l2. split. reflexivity. intros. apply H1.
+    simpl. right. assumption.
+Qed.
+
+(*Multistep version of the above*)
+Lemma first_queue_contant_multi: forall s g v v' d' l1 l2 s',
+  valid s g v ->
+  get_queue s = l1 ++ (v', d') :: l2 ->
+  (forall x, In x (map fst l1) -> x <> v') ->
+  ~In v' (map fst (get_dists s)) ->
+  bfs_multi s s' ->
+  (In (v', d') (get_dists s') \/ 
+  (~In v' (map fst (get_dists s')) /\
+  exists l1 l2, get_queue s' = l1 ++ (v', d') :: l2  /\
+  (forall x, In x (map fst l1) -> x <> v'))).
+Proof.
+  intros. generalize dependent l1. revert l2. induction H3; intros.
+  - right. split; try(assumption). exists l1. exists l2. split; try(assumption).
+  - pose proof (first_queue_constant _ _ _ _ _ _ _ _ H H1 H4 H2 H0). destruct H5.
+    left. eapply output_preserved_strong. eapply v_step. apply H. apply H0.
+    assumption. apply H5. destruct_all. assert (valid y g v). eapply v_step.
+    apply H. assumption. specialize (IHmulti H8 H5 _ _ H6 H7). apply IHmulti.
+Qed.
+
+(*Now we know that if (v', d') is the first instance of v' on the queue at some point, v', g') is in
+  the distances when we finish (since the other condition cannot happen)*)
+Lemma first_queue_in_dists: forall s g v v' d' l1 l2 s',
+  valid s g v ->
+  valid s' g v ->
+  get_queue s = l1 ++ (v', d') :: l2 ->
+  (forall x, In x (map fst l1) -> x <> v') ->
+  ~In v' (map fst (get_dists s)) ->
+  done s' = true ->
+  In (v', d') (get_dists s').
+Proof.
+  intros. destruct (done s) eqn : D.
+  - assert (s = s'). eapply done_unique. apply H. 
+    assumption. assumption. assumption. subst.
+    unfold done in D. rewrite H1 in D. rewrite orb_true_iff in D.
+    destruct D. destruct l1; simpl in H5; inversion H5.
+    rewrite isEmpty_def in H5. 
+    assert (vIn (get_graph s') v' = true). destruct (vIn (get_graph s') v') eqn : V.
+    reflexivity. eapply graph_iff_not_output in V. contradiction. apply H.
+    eapply queue_in_graph. apply H. rewrite H1. rewrite map_app. simpl. solve_in.
+    rewrite H5 in H6. inversion H6. assumption.
+  - pose proof (multi_done _ _ _ _ H H0 D H4).
+    pose proof (first_queue_contant_multi _ _ _ _ _ _ _ _ H H1 H2 H3 H5). destruct H6. assumption.
+    destruct_all. unfold done in H4. rewrite H7 in H4.
+    rewrite orb_true_iff in H4. destruct H4. destruct x; simpl in H4; inversion H4.
+    rewrite isEmpty_def in H4. destruct (vIn (get_graph s') v') eqn : V.
+    rewrite H4 in V. inversion V. eapply graph_iff_not_output in V. 
+    contradiction. apply H0. eapply queue_in_graph. apply H. rewrite H1. rewrite map_app; simpl; solve_in.
+    assumption.
+Qed.
+
+(*TODO: move to helper*)
+Lemma in_split_app_fst_map: forall {A B: Type} {Eq1: (forall x y : A, {x = y} + {x <> y})}
+   {Eq2: forall x y : B, {x = y} + {x <> y}}  (l: list (A * B)) x y,
+  In (x, y) l ->
+  (forall y', In (x, y') l -> y = y') ->
+  exists l1 l2, l = l1 ++ ((x, y) :: l2) /\ forall y, In y (map fst l1) -> y <> x.
+Proof.
+  intros. induction l.
+  - inversion H.
+  - destruct a0. simpl. destruct (Eq2 y b0). subst. destruct (Eq1 x a0). subst. exists nil.
+    exists l. split. reflexivity. intros. inversion H1. 
+    subst. simpl in H. destruct H. inversion H; subst. contradiction.
+     apply IHl in H. destruct_all.
+    exists ((a0, b0) :: x0). exists x1. split. rewrite H. reflexivity. intros. intro. subst.
+    simpl in H2. destruct H2. subst. contradiction. apply H1 in H. contradiction.
+    intros. apply H0. solve_in. destruct (Eq1 x a0). subst. assert (y = b0). apply H0.
+    simpl. left. reflexivity. subst. contradiction. simpl in H. destruct H.
+    inversion H; subst; contradiction. apply IHl in H.
+    destruct_all. exists ((a0, b0) :: x0). exists x1. split. rewrite H. simpl. reflexivity.
+    intros. simpl in H2. destruct H2. subst. intro. subst. contradiction. apply H1. assumption.
+    intros. apply H0. solve_in.
+Qed.
+
+Lemma in_split_app_special:  forall {A B: Type} {Eq1: (forall x y : A, {x = y} + {x <> y})}
+    (l: list (A * B)) x,
+  In x (map fst l) ->
+  exists y l1 l2, l = l1 ++ ((x, y) :: l2) /\ forall y, In y (map fst l1) -> y <> x.
+Proof.
+  intros. induction l.
+  - destruct H.
+  - simpl in *. destruct a0. destruct (Eq1 x a0). subst. destruct H. simpl in H. inversion H; subst. exists b0.
+    exists nil. exists l. split. reflexivity. intros. destruct H1.
+    exists b0. exists nil. exists l. split. reflexivity. intros. inversion H0.
+    destruct H. simpl in H. inversion H. subst. contradiction. 
+    apply IHl in H. destruct_all. exists x0. exists ((a0, b0) :: x1). exists x2. split. rewrite H. reflexivity.
+    intros. simpl in H1. destruct H1. subst. auto. apply H0. assumption.
+Qed.
+
+Lemma queue_smaller_than_dists: forall s g v,
+  valid s g v ->
+  (forall n, In n (map snd (get_queue s)) ->
+  (forall m, In m (map snd (get_dists s)) ->
+  (m <= n)%Z)).
+Proof.
+  intros. generalize dependent n. generalize dependent m. induction H; intros. unfold start in *; simpl in *. destruct H1.
+  inversion H0; subst; simpl in *.
+  - rewrite map_app in *. apply in_app_or in H1. apply in_app_or in H2. destruct H2.
+    destruct H1. apply IHvalid.  assumption. right. assumption. simpl in H1.
+    destruct H1. subst. pose proof (queue_structure _ _ _ v0 m vs H) .
+    assert (get_queue (g0, (v0, m) :: vs, d) = (v0, m) :: vs) by reflexivity. specialize (H1 H5); clear H5.
+    destruct H1. simpl in H1. apply Sorted_StronglySorted in H1. inversion H1; subst.
+    rewrite Forall_forall in H9. apply H9. assumption. unfold Relations_1.Transitive. intros. omega. 
+    destruct H1.  
+    rewrite in_map_iff in H2. destruct H2. destruct x. simpl in *. destruct H2. subst.  
+    rewrite (suci_def n0 n _ c v0 g0 g' H4) in H5. destruct H5. subst.
+    destruct H1. assert ( (m<=j)%Z). apply IHvalid. assumption. left. reflexivity. omega.
+    destruct H1. subst. omega. destruct H1.
+  - apply IHvalid. assumption. right. assumption.
+Qed.
+
+(*TODO: move to helper*)
+Lemma sort_app: forall {A : Type} (l1 l2 : list A) R,
+  Sorted R (l1 ++ l2) ->
+  Relations_1.Transitive R ->
+  (forall x y, In x l1 -> In y l2 -> R x y).
+Proof.
+  intros. generalize dependent l2. induction l1; intros.
+  - simpl in H. destruct H1.
+  - simpl in H. apply Sorted_StronglySorted in H. inversion H. subst.
+    rewrite Forall_forall in H6. simpl in H1.
+    destruct H1. subst. apply H6. solve_in. eapply IHl1.
+    assumption. apply StronglySorted_Sorted . apply H5.
+    assumption. assumption.
+Qed. 
+
+(*Another key property of BFS: the distances are sorted*)
+Theorem dists_sorted: forall s g v,
+  valid s g v ->
+  Sorted Z.le (map snd (get_dists s)).
+Proof.
+  intros. induction H.
+  - simpl. constructor.
+  - inversion H0; subst; simpl in *.
+    + rewrite map_app. eapply SortA_app. apply eq_equivalence. apply IHvalid.
+      simpl. constructor. constructor. constructor. intros.
+      simpl in H4. rewrite <- In_InA_equiv in H4. rewrite <- In_InA_equiv in H3. 
+      eapply queue_smaller_than_dists. apply H.
+      simpl. simpl in H4. destruct H4. subst. left. reflexivity. destruct H4.
+      simpl. assumption.
+    + assumption.
+Qed.
+
+
+(** The big result: Every (v', d) pair that appears in the output is actually the shortest
+  distance from v to v'. This also implies reachability, although that was already proved separately
+  (and is needed for this proof) **)
+
+Theorem bfs_tail_correct: forall s g v,
+  valid s g v ->
+  done s = true ->
+  (forall v',
+  vIn g v' = true ->
+  find_dist s v' = distance g v v').
+Proof.
+  intros. destruct (distance g v v') eqn : D.
+  - generalize dependent v'. induction n as [ n IHn ] using (well_founded_induction lt_wf).
+    intros. destruct (find_dist s v') as [n'|] eqn : D' .
+    rewrite find_dist_in in D'.
+    pose proof (dist_upper_bound _ _ _ _ _ H D'). rewrite D in H2.
+    rewrite Nat2Z.id in H2. simpl in H2.
+    destruct (Nat.eq_dec n n'). subst. reflexivity. rewrite Nat.leb_le in H2.
+    assert (n < n') by omega. clear n0. clear H2.
+    (*It cannot be the start node*)
+    destruct (N.eq_dec v v'). subst. unfold distance in D. rewrite distance_some in D.
+    destruct D. destruct H2. subst. pose proof (start_0_dist _ _ _ H).
+    assert (In (v', 0%Z) (get_dists s)). apply H4. intro. rewrite H5 in D'. destruct D'.
+    assert (Z.of_nat n' = 0%Z). eapply NoDup_pairs. apply   (no_dups_output _ _ _ H).
+    apply D'. assumption. assert (n' = 0) by omega. subst. omega. destruct_all. contradiction.
+    (*Get predecessor on shortest path*)
+    assert (P := D). unfold distance in P. rewrite distance_some in P. destruct P. destruct H2.
+    subst. contradiction. destruct H2. destruct H4. destruct H5.
+    destruct H5 as [l]. destruct H5. destruct l as [| w l]. simpl in H7.
+    inversion H5. subst.
+    (*TODO: see if i can do this without repeating twice*)
+    assert (n = 1) by omega. subst. clear H2. clear H7. assert (vIn g v = true).
+    eapply valid_in; apply H. pose proof (done_not_start g v H2). rewrite not_done_step in H7.
+    destruct H7 as [s2]. pose proof (second_state s2 _ _ H2 H7).
+    unfold start in H7. inversion H7; subst. simpl in *.
+    assert (valid (g', suci c 1%Z, (v, 0%Z) :: nil) g v). eapply v_step.
+    apply v_start. assumption. apply H7.
+    assert (In (v', 1%Z) (suci c 1%Z)). rewrite suci_def. split. reflexivity.
+    apply H8. apply H17. apply (@in_split_app_fst_map _ _ N.eq_dec Z.eq_dec) in H11.
+    destruct H11 as [l1]. destruct H11 as [l2]. destruct H11.
+    assert (In (v', 1%Z) (get_dists s)). eapply first_queue_in_dists. apply H10.
+    assumption. simpl. apply H11. apply H12. simpl. intro. destruct H13. subst.
+    contradiction. destruct H13. assumption.
+    pose proof (no_dups_output _ _ _ H).  
+    epose proof ((NoDup_pairs (get_dists s)) _ _ _ H14 H13 D'). omega.
+    intros. rewrite suci_def in H12. omega. apply H17.
+    rewrite <- match_in in H2. destruct_all. rewrite H2 in H17. inversion H17.
+    apply v_start. apply H2. 
+    (*Now, the case when there is an intermediate neighbor (slightly harder but the same basic idea)*)
+    inversion H5; subst.
+    assert (vIn g v = true). eapply valid_in. apply H.
+    destruct (distance g v w) as [nw|] eqn : DW . unfold distance in DW. assert (E := DW).
+    rewrite distance_some in DW. simpl in H7. destruct DW. destruct H9. symmetry in H9. subst.
+    assert (path_list g v v' nil = true). simpl. assumption. rewrite H6 in H9. inversion H9.
+    simpl. omega. assert (nw + 1 = n). { destruct_all.
+    pose proof (shortest_path_transitive g v v' (w :: l) w x nil). simpl in H16.
+    assert (S(length l) = length x + 0 + 1). apply H16. unfold shortest_path.
+    split; try(assumption). rewrite <- path_list_equiv. apply H5. intros.
+    apply H6. simpl in H17. omega. left. reflexivity. unfold shortest_path.
+    split. rewrite <- path_list_equiv. assumption. intros. apply H12. omega.
+    unfold shortest_path. split. simpl. assumption. intros. simpl in H17. omega.
+    omega. } subst. 
+    assert (find_dist s w = Some nw). apply IHn. omega. apply edges_valid in H14. destruct H14. assumption.
+    assumption. rewrite find_dist_in in H10. 
+    (*we know that the predecessor has distance 1 less and is thus in the distances correctly. We now
+    look at the state at which this vertex is added to the distances*)
+    pose proof (output_is_added _ _ _ _ _ H H10). destruct H11 as [sw]. destruct H11 as [c].
+    destruct H11 as [g']. destruct H11. destruct H12. destruct H15. destruct H16. 
+    destruct H17 as [l2]. destruct H15. destruct H15. 
+    (*first case, v' is already finished *)
+    destruct (In_dec N.eq_dec v' (map fst (get_dists sw))).
+    rewrite H17 in i. rewrite map_app in i. apply in_app_or in i. destruct i.
+    rewrite in_map_iff in H19. destruct H19. destruct x0. simpl in H19. destruct H19; subst.
+    pose proof (dists_sorted _ _ _ H11). rewrite H17 in H19. rewrite map_app in H19. 
+    simpl in H19. epose proof (sort_app (map snd l2) (Z.of_nat nw :: nil) Z.le H19).
+    assert (Relations_1.Transitive Z.le). unfold Relations_1.Transitive. intros; omega.
+    specialize (H21 H22); clear H22. specialize (H21 i (Z.of_nat nw)).
+    assert (i <= Z.of_nat nw)%Z.  apply H21. rewrite in_map_iff. exists (v', i).
+    split. reflexivity. assumption. simpl. left. reflexivity. clear H21.
+    pose proof (no_dups_output _ _ _ H). epose proof (NoDup_pairs _ v' i (Z.of_nat n') H21).
+    assert (i = Z.of_nat n'). apply H23. eapply output_preserved_strong.
+    apply H11. assumption. rewrite H17. solve_in. assumption. omega.
+    simpl in H19. destruct H19. subst. destruct_all. rewrite path_list_equiv in H20.
+    rewrite H6 in H20. inversion H20. omega. destruct H19.
+    (* Now we know that v' has not been finished already. Now we need to see if it was already in
+        the queue or not*)
+    (*Next case: v' not already done, but it is already on the queue*)
+    (*Hmm do we need that - just look at 1st position on the queue, it is <= nw + 1 by sorted, already a contradiction*)
+    simpl in H15. assert (In v' (map fst (suci c (Z.of_nat nw + 1)%Z))). { assert (vIn (get_graph sw) v' = true). 
+    destruct (vIn (get_graph sw) v') eqn : ?. reflexivity. rewrite <- graph_iff_not_output in Heqb0.
+    contradiction. apply H11. assumption.
+    pose proof suci_def. pose proof (prior_state _ _ _ H11 H16). destruct H21 as [sp]. destruct H21.
+    specialize (H18 _ H21 H22). destruct H18. destruct H23. simpl in H15. 
+    specialize (H20 v' ((Z.of_nat nw + 1)%Z) ((Z.of_nat nw + 1)%Z) c w (get_graph sp) g' H23).
+    destruct H20. rewrite in_map_iff. exists (v', (Z.of_nat nw + 1)%Z). simpl. split. reflexivity.
+    apply H25. split. reflexivity. rewrite edge_in_state. split; try(assumption).
+    rewrite <- match_in. exists c. exists g'. assumption. 
+    destruct (vIn (get_graph sp) v') eqn : V. reflexivity. rewrite <- graph_iff_not_output in V.
+    assert (In v' (map fst (get_dists sw))). eapply output_preserved. apply H21.
+    eapply multi_step. apply H22. constructor. assumption. contradiction. apply H21. assumption.
+    apply H21. assumption. }
+    assert (In v' (map fst (get_queue sw))). rewrite H15. rewrite map_app. solve_in.
+    epose proof (@in_split_app_special _ _ N.eq_dec _ _ H20). destruct H21 as [i]. 
+    destruct H21 as [l']. destruct H21 as [l'']. clear H20. assert (H20 := H21). clear H21. destruct H20.
+    assert (suci c (Z.of_nat nw + 1)%Z <> nil). 
+    destruct (suci c (Z.of_nat nw + 1)%Z) eqn : S. destruct H19. intro. inversion H22.
+    pose proof (exists_last H22). destruct H23. destruct s0. rewrite e in H15.
+    assert (Sorted Z.le (map snd (get_queue sw))). 
+    destruct l'. simpl in H20.
+    pose proof (queue_structure _ _ _ _ _ _ H11 H20). apply H23. simpl in H20. destruct p.
+    pose proof (queue_structure _ _ _ _ _ _ H11 H20). apply H23.
+    assert (i <= (Z.of_nat  nw + 1))%Z. { destruct x1. 
+    assert (In (n1, i0) (suci c (Z.of_nat nw + 1)%Z )) by (rewrite e; solve_in).
+    pose proof suci_def. pose proof (prior_state _ _ _ H11 H16). destruct H26 as [sp]. destruct H26.
+    specialize (H18 _ H26 H27). destruct H18. destruct H28. 
+    specialize (H25 n1 i0 ((Z.of_nat nw + 1)%Z) c w (get_graph sp) g' H28).
+    rewrite H25 in H24. destruct H24. subst.
+    clear H27. clear H26. clear H25. destruct l''.  rewrite H15 in H20.
+    pose proof ( app_inj_tail  (x ++ x0) l' (n1, (Z.of_nat nw + 1)%Z) (v', i)).
+    assert (x ++ x0 = l' /\ (n1, (Z.of_nat nw + 1)%Z) = (v', i)). apply H24. rewrite <- app_assoc.
+    apply H20. clear H24. destruct H25. inversion H25; subst. omega.
+    remember (p :: l'') as l'''. assert (l''' <> nil). subst. intro. inversion H24.
+    pose proof (exists_last H24). destruct H25. destruct s0. rewrite e0 in H20.
+    rewrite H15 in H20. destruct x2.
+    pose proof  ( app_inj_tail  (x ++ x0) ( l' ++ (v', i) :: x1) (n1, (Z.of_nat nw + 1)%Z) (n2, i0)).
+    assert (x ++ x0 = l' ++ (v', i) :: x1 /\ (n1, (Z.of_nat nw + 1)%Z) = (n2, i0)). apply H25.
+    rewrite <- app_assoc. rewrite H20. rewrite <- app_assoc. simpl. reflexivity. clear H25.
+    destruct H26. inversion H26; subst. rewrite app_assoc in H15. rewrite H25 in H15.
+    rewrite H15 in H23. rewrite map_app in H23. eapply sort_app in H23.
+    apply H23. unfold Relations_1.Transitive. intros. omega. rewrite map_app.
+    simpl. solve_in. simpl. left. reflexivity. }
+    pose proof (first_queue_in_dists _ _ _ _ _ _ _ _ H11 H H20 H21 n H0).
+    assert (i = Z.of_nat n'). eapply NoDup_pairs. eapply no_dups_output.
+    apply H. apply H25. assumption. subst. omega. apply H.
+    (*The hard part is over!*)
+    unfold distance in DW. rewrite distance_none in DW. destruct DW. rewrite path_list_equiv in H13.
+    rewrite H9 in H13. inversion H13. apply H.
+    rewrite find_dist_not in D'. unfold distance in D. rewrite distance_some in D.
+    destruct D. destruct_all. subst. exfalso. apply (D' 0%Z). eapply start_0_dist.
+    apply H. intro. rewrite dists_nil_iff_start in H2. 
+    assert (done s = false). rewrite H2. apply done_not_start .  apply H1.
+    rewrite H3 in H0. inversion H0. assumption. destruct_all.
+     pose proof (output_iff_reachable _ _ _ v' H H0). destruct H7.
+    assert (In v' (map fst (get_dists s))). apply H8. right.
+    exists x. assumption. exfalso. rewrite in_map_iff in H9.
+    destruct H9. destruct x0. simpl in H9; destruct H9; subst.
+    apply (D' i). assumption.
+  - pose proof (output_iff_reachable _ _ _ v' H H0).
+    unfold distance in D. rewrite distance_none in D.
+    destruct H2. apply contrapositive in H2. rewrite find_dist_not. intros.
+    intro. apply H2. rewrite in_map_iff. exists (v', y). simpl. split. reflexivity.
+    assumption. intro. destruct H4. subst. destruct_all; contradiction.
+    destruct H4. destruct D. rewrite path_list_equiv in H4. rewrite H5 in H4. inversion H4.
+Qed. 
+End Correctness.
+
+Section Equiv.
+
+(*TODO: Fix this*)
+
+
+(*
+(*Let's try it*)
+Equations bfs_queue (s: state) : state by wf (get_graph s, get_queue s) (bf_measure_list (Node * Num.Int)) :=
+  bfs_queue (g, nil, x, go) => (g, nil, x, go);
+  bfs_queue (g, (v, j) :: vs, d, go) => if (isEmpty g) then (g, (v,j) :: vs, d, go) else
+    match (match_ v g) as y return ((match_ v g = y) -> _) with
+      | (Some c, g') => fun H: (match_ v g) = (Some c, g') => 
+        bfs_queue (g', (vs ++ (filter (fun x => if (in_dec N.eq_dec (fst x) (map fst ((v,j) :: vs))) then false else true)
+       (suci c (Num.op_zp__ j (Num.fromInteger 1))))), d ++ (v,j) :: nil, go)
+      | (None, g') => fun H: (match_ v g) = (None, g') => bfs_queue (g', vs, d, go)
+      end (eq_refl).
+
+Next Obligation.
+unfold bf_measure_list. unfold transp. apply lex1. unfold natNodes_lt. eapply match_decr_size. symmetry. apply H.
+Defined.
+Next Obligation.
+unfold bf_measure_list. unfold transp. apply lex2. unfold natNodes_eq. eapply match_none_size. apply H. unfold list_length_lt.
+simpl. omega.
+Defined.
+
+Definition expand_bfs_queue := 
+fun s : gr a b * list (Node * Num.Int) * list (Node * Num.Int) * gr a b =>
+let (p, g) := s in
+(let (p0, l) := p in
+ fun g0 : gr a b =>
+ (let (g1, l0) := p0 in
+  fun (l1 : list (Node * Num.Int)) (g2 : gr a b) =>
+  match l0 with
+  | nil => fun (l2 : list (Node * Num.Int)) (g3 : gr a b) => (g1, nil, l2, g3)
+  | p1 :: l2 =>
+      fun (l3 : list (Node * Num.Int)) (g3 : gr a b) =>
+      (let (n, i) := p1 in
+       fun (l4 l5 : list (Node * Num.Int)) (g4 : gr a b) =>
+       if isEmpty g1
+       then (g1, (n, i) :: l4, l5, g4)
+       else
+        (let
+           (m, g') as y
+            return (match_ n g1 = y -> gr a b * list (Node * Num.Int) * list (Node * Num.Int) * gr a b) :=
+           match_ n g1 in
+         match
+           m as m0
+           return (match_ n g1 = (m0, g') -> gr a b * list (Node * Num.Int) * list (Node * Num.Int) * gr a b)
+         with
+         | Some c =>
+             fun _ : match_ n g1 = (Some c, g') =>
+             bfs_queue
+               (g',
+               l4 ++
+               filter
+                 (fun x : N * Num.Int =>
+                  if in_dec N.eq_dec (fst x) (map fst ((n, i) :: l4)) then false else true)
+                 (suci c (Num.op_zp__ i (Num.fromInteger 1))), l5 ++ (n, i) :: nil, g4)
+         | None => fun _ : match_ n g1 = (None, g') => bfs_queue (g', l4, l5, g4)
+         end) eq_refl) l2 l3 g3
+  end l1 g2) l g0) g.
+
+Lemma unfold_bfs_queue: forall s,
+  bfs_queue s = expand_bfs_queue s.
+Proof.
+  intros. unfold expand_bfs_queue. apply bfs_queue_elim; intros; reflexivity.
+Qed.
+
+(*Let's see...*)
+
+(*Show that if s --> done state, and steps to another, then unique*)
+(*show that every done, valid state is unique*)
+(*Then, show that every state multisteps to a done, valid state (done)*)
+(*So, then show that if we take a state, remove duplicates from its queue, then it multisteps to a valid done state*)
+
+Lemma done_cannot_step: forall s s',
+  bfs_step s s' ->
+  done s = false.
+Proof.
+  intros. unfold done. inversion H; subst; simpl; assumption.
+Qed.
+
+(*Maybe, alternate*)
+(*For every element in the queue, there is a state you multistep to where that element is at the front of the queue*)
+(*And they occur in order*)
+(**)
+
+(*Let's try with map solution*)
+
+
+Lemma queue_remove_dup_single: forall g q d go v s' l1 l2 l3 v' d' d'',
+  q = l1 ++ (v', d') :: l2 ++ (v', d'') :: l3 ->
+  done (g, q, d, go) = false ->
+  valid (g, q, d, go) v ->
+  bfs_multi (g, q, d, go) s' ->
+  done s' = true ->
+  bfs_multi (g, l1 ++ (v', d') :: l2 ++ l3, d, go) s'.
+Proof.
+  intros. remember (g, q, d, go) as s. generalize dependent l1. revert l2. revert l3. revert v'. revert d'.
+  revert d''. generalize dependent q. revert g. revert d. revert go. induction H1; intros; subst.
+  - unfold start in Heqs. inversion Heqs; subst. destruct l1; inversion H5; subst. 
+    destruct l2; inversion H7. destruct l1; inversion H6.
+  - assert (done s'0 = false) by (eapply done_cannot_step; apply H). specialize (IHvalid H4). clear H4.
+    assert (bfs_multi s'0 s'). eapply multi_step. apply H. apply H2. specialize (IHvalid H4). clear H4.
+    inversion H; subst; simpl in *.
+    + eapply IHvalid. reflexivity. unfold done in H0. simpl in H0.
+
+  inversion H4; subst; simpl in *.
+    + 
+    inversion H5; subst. 
+
+
+ induction H1; subst.
+  - unfold start in Heqs. inversion Heqs. subst.  unfold done in H2. simpl in H2. destruct l1; simpl in H2. simpl in H2.
+  - 
+  
+
+Lemma queue_remove_dup: forall 
+
+Lemma queue_equiv: forall s,
+  bfs_tail s = bfs_queue s.
+Proof.
+  intros. destruct s as [r go]. destruct r as [r d]. revert d. revert go.
+  induction (r) using (well_founded_induction (well_founded_bf_measure_list (Node * Num.Int))).
+  intros. destruct r as [g q]. rewrite unfold_bfs_tail. rewrite unfold_bfs_queue. simpl.
+  destruct q.
+  - reflexivity.
+  - destruct p. destruct (isEmpty g) eqn : E.
+    + reflexivity.
+    + destruct (match_ n g) eqn : M. destruct m.
+      * 
+
+*)
+(*Want to prove this is valid, done and equivalent to other*)
+
+(*
 (*Equivalence of 2 versions - TODO: prove leveln and leveln' equivalent (proof is basically what I did before*)
 Equations leveln' (x: (gr a b) * (list (Node * Num.Int))) : list (Node * Num.Int) by wf x (bf_measure_list (Node * Num.Int)) :=
   leveln' (g, nil) := nil;
@@ -720,8 +2142,8 @@ Proof.
   intros. unfold expand_leveln'. apply leveln'_elim. reflexivity. reflexivity.
 Qed.
 
-Lemma leveln_tail_equiv: forall x l n t,
-  get_dists (bfs_tail (x, l, n, t)) = l ++ leveln' x.
+Lemma leveln_tail_equiv: forall x l go,
+  get_dists (bfs_tail (x, l, go)) = l ++ leveln' x.
 Proof.
   intros x. 
   induction (x) using (well_founded_induction (well_founded_bf_measure_list (Node * Num.Int))).
@@ -907,10 +2329,7 @@ Proof.
   intros. pose proof (bf_list_equiv (g, q)). simpl in H. assumption.
 Qed. 
 
-Lemma contrapositive: forall (P Q : Prop), (P -> Q) -> (~Q -> ~P).
-Proof.
-  tauto.
-Qed. 
+
 (*probably dont need this*)
 Lemma bf_list_unroll: forall (g: gr a b) (l: list Path) n p t,
   l = (n :: p) :: t ->
@@ -939,4 +2358,7 @@ End WithPath.
 5. need something about the paths, tail vs regular recursive*)
 
 (*Next step: try to prove this is equivalent to Haskell BFS, then can just work with this version/ valid states*)
+
+*)
+End Equiv.
 End Ind.
