examples/graph/theories/Helper.v
@@ -1,0 +1,62 @@
+Require Import Coq.Bool.Bool.
+Require Import Coq.Lists.List.
+Require Import Coq.Lists.ListDec.
+(*Helper Lemmas and tactics*)
+
+Definition null {a} (l: list a) :=
+  match l with
+  | nil => true
+  | _ => false
+  end.
+
+Ltac simplify' := try(rewrite andb_diag in *); try(rewrite andb_true_iff in *); try(rewrite negb_true_iff in *);
+  try(rewrite andb_false_iff in *); try(rewrite negb_false_iff in *); intuition.
+
+Ltac destruct_all :=
+repeat(match goal with
+            |[H: (exists _, _) |- _] => destruct H
+            |[H: _ /\ _ |- _] => destruct H 
+            end; try(rewrite andb_true_iff in *)).
+
+(*Ltac for solving statements of the form: In x l, where l may be many lists appended together*) 
+Ltac solve_in :=
+  match goal with
+  | [ H : _ |- In ?x (?l ++ ?r)] => apply in_or_app; solve_in
+  | [ H : _ |- In ?x ?s \/ In ?x ?s'] => (right; solve_in) + (left; solve_in) 
+  | [ H : _ |- In ?x (?x :: ?l)] => simpl; left; reflexivity
+  | [H : _ |- In ?x (?a :: ?l)] => simpl; right; solve_in
+  | [ H : _ |- _ ] => try(reflexivity); assumption
+end. 
+
+Lemma in_split_app_fst: forall (A: Type) (l: list A) (x: A),
+  (forall x y : A, {x = y} + {x <> y}) ->
+  In x l ->
+  exists l1 l2, l = l1 ++ (x :: l2) /\ forall y, In y l1 -> y <> x.
+Proof.
+  intros. induction l.
+  - inversion H.
+  - destruct (X x a). subst. exists nil. exists l. split. reflexivity. intros. inversion H0.
+    simpl in H. destruct H. subst. contradiction.  apply IHl in H. destruct_all.
+    exists (a :: x0). exists x1. split. rewrite H. reflexivity. intros. intro. subst.
+    simpl in H1. destruct H1. subst. contradiction. apply H0 in H. contradiction.
+Qed.
+
+Lemma no_no_dup: forall (A: Type) (l: list A),
+  (forall x y : A, {x = y} + {x <> y}) ->
+  ~(NoDup l) <-> (exists w l1 l2 l3, l = l1 ++ w :: l2 ++ w :: l3).
+Proof.
+  intros. split; intros.
+  - induction l.
+    + assert (@NoDup A nil). constructor. contradiction.
+    + destruct (NoDup_dec X l).
+      * assert (In a l). destruct (In_dec X a l). apply i.
+        assert (NoDup (a :: l)). constructor. apply n0. apply n. contradiction.
+        apply in_split_app_fst in H0. destruct_all. exists a. exists nil. exists x. exists x0.
+        rewrite H0. reflexivity. apply X.
+      * apply IHl in n. destruct_all. exists x. exists (a :: x0). exists x1. exists x2. rewrite H0.
+        reflexivity.
+  -  intro. destruct_all.  subst. induction x0; simpl in *.
+    + rewrite NoDup_cons_iff in H0. destruct_all. apply H.
+    solve_in.
+    + simpl in H0. rewrite NoDup_cons_iff in H0. destruct_all. apply IHx0. apply H0.
+Qed.
