examples/graph/theories/Path.v
@@ -1,0 +1,367 @@
+Require Import Data.Graph.Inductive.Graph.
+Require Import Coq.Lists.List.
+Require Import Coq.Bool.Bool.
+Require Import Helper.
+Require Import Wellfounded.
+Require Import Coq.Lists.ListDec.
+Require Import Coq.NArith.BinNat.
+Require Import Omega.
+Require Import Crush.
+
+(*Lots of stuff about paths here*)
+Section Path.
+
+Context {a : Type} {b : Type} { gr : Type -> Type -> Type} {Hgraph : Graph.Graph gr} {Hlaw : Graph.LawfulGraph gr}.
+
+(*Inductive and Fixpoint definitions for a path between two vertices. The Fixpoint instance proves that this is
+  decidable, and we prove their equivalence*)
+Inductive path : (gr a b) -> Node -> Node -> (list Node) -> Prop :=
+  | p_start: forall g u v, eIn g u v = true -> path g u v nil
+  | p_step: forall g u v w l, 
+     path g u w l ->
+     eIn g w v = true ->
+     path g u v (w :: l) .
+
+Fixpoint path_list (g: gr a b) (u v: Node) (l: list Node) : bool :=
+  match l with
+  | nil => eIn g u v
+  | x :: tl => eIn g x v && path_list g u x tl
+  end.
+
+Lemma path_list_equiv: forall g u v l,
+  path g u v l <-> path_list g u v l = true.
+Proof.
+  intros. split; intros.
+  - induction H.
+    + simpl. assumption.
+    + simpl. rewrite andb_true_iff. split; assumption.
+  - generalize dependent v. induction l; intros; simpl.
+    + apply p_start. simpl in H. assumption.
+    + simpl in *. rewrite andb_true_iff in H. destruct H. apply p_step. apply IHl. assumption.
+      assumption.
+Qed.
+
+(*Some useful results about [path]*)
+Lemma path_app: forall g u v a l1 l2,
+  path_list g u v (l1 ++ a :: l2) = true <->
+  path_list g a v l1 = true /\ path_list g u a l2 = true.
+Proof.
+  intros. split; intros. generalize dependent v. generalize dependent l2. induction l1; intros.
+  - simpl in H. simpl. rewrite andb_true_iff in H. apply H.
+  - simpl in *. simplify'; apply IHl1 in H1; destruct H1; assumption.
+  - destruct_all. generalize dependent v. generalize dependent a0. revert l2. induction l1; intros; simpl in *;
+    simplify'.
+Qed.
+
+Lemma path_remove_cycle: forall g u v w l1 l2 l3,
+  path_list g u v (l1 ++ w :: l2 ++ w :: l3) = true ->
+  path_list g u v (l1 ++ w :: l3) = true.
+Proof.
+  intros. apply path_app in H. destruct_all. apply path_app in H0. destruct_all.
+  apply path_app. simplify'.
+Qed.
+
+(*If there is a path, then there is a path with no duplicates*)
+Lemma path_no_dups: forall g u v l,
+  path_list g u v l = true ->
+  exists l1, path_list g u v l1 = true /\ NoDup l1 /\ ~In u l1 /\  ~In v l1 /\ 
+  (forall x, In x l1 -> In x l). 
+  Proof.
+    intros. induction l using (well_founded_induction
+                       (wf_inverse_image _ nat _ (@length _)
+                          PeanoNat.Nat.lt_wf_0)).
+    destruct (NoDup_dec (N.eq_dec) l).
+    - destruct (In_dec N.eq_dec u l).
+      + eapply in_split_app_fst in i. destruct_all. clear H2. subst.
+        apply path_app in H. destruct H. specialize (H0 x). destruct H0 as [l]. 
+        rewrite app_length. simpl. assert (forall n m, n < n + S(m)) by (intros; omega). apply H0.
+        apply H. exists l. simplify'. apply N.eq_dec.
+      + destruct (In_dec N.eq_dec v l).
+        * eapply in_split_app_fst in i. destruct_all; subst. clear H2. apply path_app in H.
+          destruct H. specialize (H0 x0). destruct H0 as [l]. rewrite app_length. simpl.
+          assert (forall n m, n < m + S(n)) by (intros; omega). apply H0. apply H1. exists l.
+          simplify'. apply N.eq_dec.
+        * exists l. simplify'.
+    - rewrite no_no_dup in n. destruct_all. subst. 
+      apply path_remove_cycle in H. specialize (H0 (x0 ++ x :: x2)). destruct H0 as [l].
+      repeat(rewrite app_length; simpl). omega. apply H. exists l. simplify'. apply H5 in H4.
+      apply in_app_or in H4. destruct H4. apply in_or_app. left. apply H4. simpl in H4.
+      destruct H4. subst. solve_in. solve_in. apply N.eq_dec.
+Qed.
+
+Lemma path_implies_in_graph: forall g u v l,
+  path_list g u v l = true ->
+  vIn g u = true /\ vIn g v = true /\ (forall x, In x l -> vIn g x = true).
+Proof.
+  intros. generalize dependent v. induction l; intros; simpl in H.
+  - apply edges_valid in H. simplify'.
+  - rewrite andb_true_iff in H. destruct H. apply IHl in H0. apply edges_valid in H. crush.
+Qed. 
+
+
+(*We want a function to get the distance between two nodes. This is a horribly inefficient function to help do this*)
+(*A terrible function to find if a path of length <= n between two vertices exists*)
+Fixpoint path_of_length (g: gr a b) (u v : Node) (n: nat) {struct n} : bool :=
+  match n with
+  | 0 => eIn g u v
+  | S(m) => if eIn g u v then true else
+  fold_right (fun x t => if path_of_length g u x m && eIn g x v then true else t) false 
+  (nodeList g)
+  end.
+
+Lemma path_of_length_implies_path: forall g u v n,
+  path_of_length g u v n = true -> exists l, path_list g u v l = true /\ length l <= n.
+Proof.
+  intros. generalize dependent v. induction n; intros.
+  - simpl in H. exists nil. split. simpl. assumption. simpl. omega.
+  - simpl in H. destruct (eIn g u v) eqn : ?.
+    exists nil. split. simpl. assumption. simpl. omega.
+    assert (forall l, fold_right
+      (fun (x : Node) (t : bool) => if path_of_length g u x n && eIn g x v then true else t) false
+      l = true-> exists x, In x l /\ path_of_length g u x n = true /\ eIn g x v = true). {
+      intros. induction l; simpl in *.
+      * inversion H0.
+      * destruct (path_of_length g u a0 n && eIn g a0 v) eqn : ?.
+        -- exists a0. split. left. reflexivity. rewrite andb_true_iff in Heqb1. apply Heqb1.
+        -- apply IHl in H0. destruct H0. exists x. destruct H0. split. right. assumption.
+           apply H1. } 
+      apply H0 in H. clear H0. destruct H. destruct H. destruct H0. apply IHn in H0.
+      destruct H0. destruct H0. exists (x :: x0). split. simpl. rewrite andb_true_iff. crush. simpl. omega.
+Qed.
+
+Lemma path_of_size_implies_function: forall g u v l n,
+  length l <= n ->
+  path_list g u v l = true -> path_of_length g u v n = true.
+Proof.
+  intros. generalize dependent v. revert u. generalize dependent n. induction l; simpl in *; intros.
+  - destruct n. simpl. apply H0. simpl. rewrite H0. reflexivity.
+  - simplify'. destruct n. omega. assert (length l <= n) by omega. clear H.
+    simpl. destruct (eIn g u v) eqn : ?. reflexivity.
+      assert (forall a l', In a l' ->
+      path_of_length g u a n = true ->
+      eIn g a v = true ->
+      fold_right
+  (fun (x : Node) (t : bool) => if path_of_length g u x n && eIn g x v then true else t)
+  false l' = true). { intros. induction l'; simpl in *.
+  - destruct H.
+  - destruct H. subst. rewrite H3. simpl. rewrite H4. simpl. reflexivity. apply IHl' in H. 
+    destruct (path_of_length g u a2 n && eIn g a2 v). reflexivity. apply H. }
+    apply (H a0). assert (vIn g a0 = true). { apply edges_valid in H1. apply H1. } unfold vIn in H3.
+    unfold mem in H3. match goal with | [H: (if ?x then _ else _) = _  |- _] => destruct x eqn : ? end.
+    assumption. inversion H3.  apply IHl. assumption. simplify'. simplify'.
+Qed.
+
+(*If there is a path, then there is a path at most as large as the number of vertices in the graph (because
+  there is a path with no duplicates and every vertex is in the graph*)
+Lemma path_shorter_than_graph_size: forall g u v l,
+  path_list g u v l = true ->
+  exists l', path_list g u v l' = true /\ length l' <= length(nodeList g).
+Proof.
+  intros. apply path_no_dups in H. destruct_all. 
+  assert (forall a, In a x -> In a (nodeList g)). intros.
+  apply path_implies_in_graph in H. destruct_all. apply H6 in H4. unfold vIn in H4.
+  unfold mem in H4.  match goal with | [H: (if ?x then _ else _) = _  |- _] => destruct x eqn : ? end.
+  assumption. inversion H4. 
+  exists x. split. apply H. eapply NoDup_incl_length. apply H0. unfold incl. apply H4.
+Qed.
+
+Definition natNodes (g : gr a b) := (BinInt.Z.abs_nat(Graph.noNodes g)).
+
+(*By the above lemma, we can simply define distance by repeatedly checking if there is a list with 
+  the given distance*)
+Definition distance (g: gr a b) (u v : Node) : option nat :=
+  if (N.eq_dec u v) then (Some 0) else
+  fold_right (fun x acc => if path_of_length g u v x then Some (x + 1) else acc) None (seq 0 (natNodes g + 1)).
+
+Lemma distance_none: forall g u v,
+  distance g u v = None <-> (forall l, path_list g u v l = false) /\ u <> v.
+Proof.
+  intros.  assert (A: forall l, fold_right (fun (x : nat) (acc : option nat) => 
+    if path_of_length g u v x then Some (x + 1) else acc) None l = None <->
+    (forall x, In x l -> path_of_length g u v x = false)). { intros. split; intros; induction l; simpl in *.
+    destruct H0. destruct H0. subst. destruct (path_of_length g u v x) eqn : ?. inversion H.
+    reflexivity. apply IHl. destruct (path_of_length g u v a0) eqn : ?. inversion H.
+    apply H. assumption. reflexivity. destruct (path_of_length g u v a0) eqn : ?.
+    specialize (H a0). rewrite H in Heqb0. inversion Heqb0. left. reflexivity.
+    apply IHl. intros. apply H. right. assumption. } 
+     split; intros.
+  - unfold distance in H. destruct (N.eq_dec u v). inversion H. split. intros. 
+    assert (forall x, In x (seq 0 (natNodes g + 1)) -> path_of_length g u v x = false). { intros.
+    eapply A.  apply H. assumption. } clear H. clear A.
+    destruct (path_list g u v l) eqn : P.
+    + apply path_shorter_than_graph_size in P. destruct P. destruct H.
+      assert (path_of_length g u v (length x) = true). eapply path_of_size_implies_function.
+      reflexivity. assumption. 
+      assert (In (length x) (seq 0 (natNodes g + 1))). apply in_seq. split. omega. simpl.
+      assert (length (nodeList g) = natNodes g). unfold natNodes. rewrite noNodes_def. 
+      unfold nodeList. unfold ulabNodes. apply map_length. omega. 
+      apply H0 in H3. rewrite H3 in H2. inversion H2.
+    + reflexivity.
+    + assumption.
+  - unfold distance. destruct (N.eq_dec u v). subst. destruct H. contradiction.
+    apply A. intros. destruct (path_of_length g u v x) eqn : ?.
+    + apply path_of_length_implies_path in Heqb0. destruct Heqb0. destruct H1. destruct H. rewrite H in H1.
+      inversion H1.
+    + reflexivity.
+Qed.
+
+Lemma seq_pred: forall start len h t n l,
+  seq start len = (h :: t) ++ S n :: l ->
+  In n (h :: t).
+Proof.
+  intros. generalize dependent h. revert t. revert start. induction len; intros.
+  - simpl. simpl in H. inversion H.
+  - simpl in H. inversion H. subst. destruct t.
+    simpl in H2. simpl. destruct len. simpl in H2. inversion H2. simpl in H2. inversion H2. subst. left. reflexivity.
+    apply IHlen in H2. solve_in.
+Qed.
+
+Lemma seq_split: forall start len l1 x l2,
+  seq start len = l1 ++ x :: l2 ->
+  (forall y, In y l1 -> y < x) /\ (forall y, In y l2 -> y > x).
+Proof.
+  intros. generalize dependent start. revert l1. revert x. revert l2. induction len; intros; simpl in H.
+  - assert (l1 = nil). destruct l1; inversion H. subst.
+    simpl in H. inversion H.
+  - destruct l1. simpl in H. inversion H. destruct l2.
+     split; intros. destruct H0. rewrite H2 in H0. destruct H0.
+     specialize (IHlen l2 n nil (S(start))). subst. simpl in IHlen. apply IHlen in H2.
+     split; intros. destruct H0. rewrite in_seq in H0. omega.
+     inversion H; subst. specialize (IHlen l2 x l1 (S(n)) H2). split; intros. simpl in H0.
+     destruct H0. subst. assert (In x (seq (S(y)) len)). rewrite H2. solve_in. rewrite in_seq in H0.
+      omega. destruct IHlen. apply H1. assumption. apply IHlen. apply H0.
+Qed.
+
+Lemma distance_neq: forall g u v n,
+  u <> v ->
+  distance g u v = Some n ->
+  n > 0.
+Proof.
+  intros. unfold distance in H0. destruct (N.eq_dec u v). subst. contradiction.
+  induction (seq 0 (natNodes g + 1)).
+  - simpl in H0. inversion H0.
+  - simpl in H0. destruct (path_of_length g u v a0) eqn : ?. inversion H0; subst; omega.
+    apply IHl. assumption.
+Qed.
+  
+
+(*This actually computes the shortest path*)
+Lemma distance_some: forall g u v n,
+  distance g u v = Some n <->
+  ((u = v /\ n = 0)) \/ (n > 0 /\ u <> v /\ (exists l, path g u v l /\ length l = (n - 1)) /\ (forall l, length l < (n - 1) -> path_list g u v l = false)).
+Proof.
+  intros. 
+  assert (forall l n, 
+  fold_right (fun (x : nat) (acc : option nat) => if path_of_length g u v x then Some (x +1) else acc) None
+  l = Some (n + 1) <-> (exists l1 l2, l = l1 ++ n :: l2 /\ (forall y, In y l1 -> path_of_length g u v y = false) /\
+  path_of_length g u v n  = true)). { intros. induction l; split; intros; simpl in *.
+  - inversion H.
+  - destruct_all. destruct x; inversion H.
+  - destruct (path_of_length g u v a0) eqn : ?. 
+    + inversion H; subst. exists nil. exists l. split. simpl. 
+      assert (a0 = n0) by omega. subst. reflexivity. split; intros.
+      destruct H0. assert (a0 = n0). omega. subst. assumption. 
+    + apply IHl in H. destruct H. exists (a0 :: x). destruct_all.
+      exists x0. split. rewrite H. simpl. reflexivity.
+      split; intros. simpl in H2. destruct H2. subst. assumption. apply H0. assumption.
+      assumption.
+  - destruct_all. destruct (path_of_length g u v a0) eqn : ?. destruct x.
+    + inversion H; subst. reflexivity. 
+    + simpl in H0. inversion H; subst. specialize (H0 n1). rewrite H0 in Heqb0. inversion Heqb0.
+      left. reflexivity.
+    + destruct x. inversion H; subst. rewrite Heqb0 in H1. inversion H1.
+      inversion H; subst. apply IHl. exists x. exists x0. simplify'. }
+   destruct (N.eq_dec u v).
+   - unfold distance. subst. destruct (N.eq_dec v v ). 
+    split; intros. inversion H0. subst. left. split; reflexivity. 
+   destruct H0. destruct H0; subst; reflexivity. destruct_all; contradiction. contradiction.
+  - split; intros. pose proof (distance_neq _ _ _ _ n0 H0). assert (exists m, m + 1 = n). {
+    exists (n - 1). omega. } destruct H2 as [m]. subst.
+    right. unfold distance in H0. destruct (N.eq_dec u v). inversion H0. 
+    rewrite <- H3 in H1. exfalso. omega.  
+    rewrite H in H0. destruct_all. clear H. split; try(assumption). split; try(assumption).
+    apply path_of_length_implies_path in H3. split. setoid_rewrite path_list_equiv. 
+    destruct  H3. destruct H. assert (length x1 = m \/ length x1 < m) by omega. destruct H4.
+    exists x1. split. assumption. omega.  
+    destruct x. simpl in H. assert (natNodes g + 1 = S(natNodes g)) by omega. rewrite H5 in H0.
+    simpl in H0. inversion H0; subst. omega. 
+    destruct m. omega. assert (length x1 <= m) by omega. assert (A:=H). 
+    apply (path_of_size_implies_function _ _ _ _ _ H5) in H. exists x1.
+    split. assumption. rewrite H2 in H. inversion H.
+    pose proof seq_pred. eapply H6. apply H0.
+    intros.   assert (In (length l) (seq 0 (natNodes g + 1))). { rewrite in_seq.
+    assert (In m (seq 0 (natNodes g + 1))). rewrite H0. solve_in. rewrite in_seq in H4.
+    omega. } rewrite H0 in H4. apply seq_split in H0. 
+    destruct H0. apply in_app_or in H4. destruct H4. 
+    destruct (path_list g u v l) eqn : ?. eapply path_of_size_implies_function in Heqb0.
+    rewrite (H2 (length l)) in Heqb0. inversion Heqb0.
+    assumption. omega. reflexivity. simpl in H4. destruct H4. omega.
+    apply H5 in H4. omega. destruct H0. destruct H0; contradiction. destruct_all.
+    assert (exists m, m + 1 = n). exists (n-1). omega. destruct H5 as [m]. subst.
+    assert (length x = m ) by omega. clear H4. unfold distance. destruct (N.eq_dec u v). subst. contradiction.
+    clear n. rewrite H. 
+    assert (m <= (natNodes g)). { assert (m <= natNodes g \/ m > natNodes g) by omega. destruct H4.
+    assumption. rewrite path_list_equiv in H2. apply path_shorter_than_graph_size in H2.
+    destruct H2. destruct H2. rewrite H3 in H2. inversion H2. unfold nodeList in H6.
+    unfold ulabNodes in H6. rewrite map_length in H6. rewrite <- noNodes_def in H6.
+    unfold natNodes in H4. omega. }
+    pose proof (in_split_app_fst _ (seq 0 (natNodes g + 1)) m Nat.eq_dec).
+    assert (In m (seq 0 (natNodes g + 1))). rewrite in_seq. omega.
+    apply H6 in H7. clear H6. destruct_all. exists x0. exists x1. split. assumption.
+    apply seq_split in H6. split; intros.
+    destruct H6. destruct (path_of_length g u v y) eqn : ?.
+    apply path_of_length_implies_path in Heqb0. destruct Heqb0.
+    destruct H10. rewrite H3 in H10. inversion H10. apply H6 in H8. omega. reflexivity.
+    eapply path_of_size_implies_function. assert (length x <= m) by omega. apply H8.
+    rewrite <- path_list_equiv. assumption.
+Qed.
+
+(* Key property of shortest paths - if u -> v is a shortest path passing through w, 
+  then the length is the shortest path from u to w + the shortest path from w to v (plus 1)*)
+Definition shortest_path g u v l :=
+  path_list g u v l = true /\ (forall l', length l' < length l -> path_list g u v l' = false). 
+
+Lemma shortest_path_transitive: forall g u v l w l' l'',
+  shortest_path g u v l ->
+  In w l ->
+  shortest_path g u w l' ->
+  shortest_path g w v l'' ->
+  length l = length l' + length l'' + 1.
+Proof.
+  intros. unfold shortest_path in *. destruct_all.
+  assert (length l < length l' + length l'' + 1 \/
+  length l > length l' + length l'' + 1 \/ length l = length l' + length l'' + 1) by omega.
+  destruct H6. apply in_split_app_fst in H0. destruct_all.
+  rewrite H0 in H. apply path_app in H. destruct H.
+  assert (length l = length x + length x0 + 1). rewrite H0. rewrite app_length.
+  simpl. omega. rewrite H9 in H6. 
+  assert (length x + length x0 < length l' + length l'') by omega. clear H6. clear H9.
+  assert (length x < length l'' \/ length x0 < length l') by omega. destruct H6.
+  rewrite H3 in H. inversion H. assumption.
+  rewrite H4 in H8. inversion H8. assumption. apply N.eq_dec.
+  destruct H6. assert (path_list g u v (l'' ++ w :: l') = true).
+  rewrite path_app. split; assumption. rewrite H5 in H7.
+  inversion H7. rewrite app_length. simpl. omega. assumption.
+Qed.
+
+(*Decidability of [path]*)
+
+Lemma path_equiv: forall g u v,
+  (exists l, path g u v l) <-> path_of_length g u v (length(nodeList g)) = true.
+Proof.
+  intros. split; intros.
+  - setoid_rewrite path_list_equiv in H. destruct H. apply path_shorter_than_graph_size in H.
+    destruct_all. eapply path_of_size_implies_function. apply H0. apply H.
+  - setoid_rewrite path_list_equiv. pose proof (path_of_length_implies_path _ _ _ _ H).
+    destruct_all. exists x. assumption. 
+Qed.
+
+Lemma path_dec: forall g u v,
+  {exists l, path g u v l} + {~exists l, path g u v l}.
+Proof.
+  intros. destruct (path_of_length g u v (length(nodeList g))) eqn : ?.
+  left. apply path_equiv; assumption.
+  right. intro. apply path_equiv in H. rewrite H in Heqb0. inversion Heqb0.
+Qed.
+
+End Path. 
